Update

HoTTModel/DTT/PTS.lean
@@ -41,70 +41,117 @@ notation N" ↑ "i => lift i 0 N
 
 variable {M N : PTerm S}
 
-def lift_inj {i c : ℕ} :
-    (M ↑ i # c) = (N ↑ i # c) → M = N := by
-  intro h
-  induction M generalizing N c with
-  | var n =>
-      simp at h
-      split_ifs at h with h₀
-      . cases N
-        all_goals simp at h
-        rename ℕ => k
-        have : k < c := by
-          split_ifs at h
-          . assumption
-          . simp at h; simp [h] at h₀; exact lt_of_le_of_lt (Nat.le_add_right _ _) h₀
-        simp [this] at h; simpa
-      . cases N
-        all_goals simp at h
-        rename ℕ => k
-        have : ¬ k < c := by
-          split_ifs at h
-          . simp at h h₀ ⊢; simp [← h]; exact h₀.trans (Nat.le_add_right _ _)
-          . assumption
-        simp [this] at h; simpa
-  | sort =>
-      cases N; all_goals simp at h
-      split_ifs at h
-      simp [h]
-  | app _ _ ih₁ ih₂ =>
-      cases N; all_goals simp at h
-      split_ifs at h
-      simpa using ⟨ih₁ h.1, ih₂ h.2⟩
-  | pi  _ _ ih₁ ih₂ =>
-      cases N; all_goals simp at h
-      split_ifs at h
-      simpa using ⟨ih₁ h.1, ih₂ h.2⟩
-  | abs  _ _ ih₁ ih₂ =>
-      cases N; all_goals simp at h
-      split_ifs at h
-      simpa using ⟨ih₁ h.1, ih₂ h.2⟩
+lemma lift_eq_var_lift {i c k : ℕ} :
+  ∀ {M : PTerm S}, (M ↑ i # c) = ((#k) ↑ i # c) → M = #k
+| .var l, h => by
+  simp at h
+  split_ifs at h with h₀ h₁ h₁
+  . assumption
+  . simp at h; simp [h] at h₀
+    simpa using not_lt_of_le (Nat.le_add_right k i) $ lt_of_lt_of_le h₀ (le_of_not_lt h₁)
+  . simp at h; simp [← h] at h₁
+    simpa using not_lt_of_le (Nat.le_add_right l i) $  lt_of_lt_of_le h₁ (le_of_not_lt h₀)
+  . simpa using h
+| .sort _, h => by simp at h; split_ifs at h
+| .app _ _, h => by simp at h; split_ifs at h
+| .abs _ _, h => by simp at h; split_ifs at h
+| .pi _ _, h => by simp at h; split_ifs at h
 
-def lift0_inj {i : ℕ} :
+lemma lift_inj {i c : ℕ} {M : PTerm S}:
+  ∀ {N : PTerm S}, (M ↑ i # c) = (N ↑ i # c) → M = N
+| .var _, h => lift_eq_var_lift h
+| .sort _, h => by
+  cases M; all_goals simp at h
+  split_ifs at h; simpa
+| .app _ _, h => by
+  cases M; all_goals simp at h
+  split_ifs at h
+  simpa using ⟨lift_inj h.1, lift_inj h.2⟩
+| .abs _ _, h => by
+  cases M; all_goals simp at h
+  split_ifs at h
+  simpa using ⟨lift_inj h.1, lift_inj h.2⟩
+| .pi _ _, h => by
+  cases M; all_goals simp at h
+  split_ifs at h
+  simpa using ⟨lift_inj h.1, lift_inj h.2⟩
+
+lemma lift0_inj {i : ℕ} :
     (M ↑ i) = (N ↑ i) → M = N :=
   lift_inj
 
-def lift_zero {c : ℕ} :
-    (M ↑ 0 # c) = M := by
-  induction M generalizing c
-  all_goals simp
-  all_goals rename_i ih₁ ih₂
-  all_goals exact ⟨ih₁, ih₂⟩
+@[simp]
+lemma lift_zero {c : ℕ} :
+    ∀ {M : PTerm S}, (M ↑ 0 # c) = M
+| .var _ => by simp
+| .sort _ => by simp
+| .app _ _ => by simp [lift_zero]
+| .abs _ _ => by simp [lift_zero]
+| .pi _ _ => by simp [lift_zero]
 
-def lift_lift (i j k : ℕ) :
-    ((M ↑ j # i) ↑ k # (j + i)) = M ↑ (j + k) # i := by
-  sorry
+lemma lift_lift (i j k : ℕ) :
+    ∀ {M : PTerm S}, ((M ↑ j # i) ↑ k # (j + i)) = M ↑ (j + k) # i
+| .var _ => by
+  simp
+  split_ifs with h
+  . simp only [lift]
+    rw [if_pos]
+    apply lt_of_lt_of_le h (Nat.le_add_left _ _)
+  . simp
+    rw [if_neg, Nat.add_assoc]
+    simpa [Nat.add_comm j i] using h
+| .sort _ => by simp
+| .app _ _ => by simp [lift_lift]
+| .abs M N => by simp [Nat.add_assoc j i 1, lift_lift]
+| .pi _ _ => by simp [Nat.add_assoc j i 1, lift_lift]
 
-def lift_lift_of_le (i j k n : ℕ) :
-    i ≤ n → ((M ↑ j # i) ↑ k # (j + n)) = (M ↑ k # n) ↑ j # i := by
-  sorry
+lemma lift_lift_of_le (i j k n : ℕ) (h : i ≤ n) :
+    ∀ {M : PTerm S}, ((M ↑ j # i) ↑ k # (j + n)) = (M ↑ k # n) ↑ j # i
+| .var m => by
+  simp
+  split_ifs with h₁ h₂ h₃
+  . simp only [lift, if_pos h₁, if_pos (lt_of_lt_of_le h₂ (Nat.le_add_left _ _))]
+  . simpa using lt_of_le_of_lt (le_of_not_lt h₂) (lt_of_lt_of_le h₁ h)
+  . simp only [lift]
+    rw [if_neg h₁, if_pos (by simpa [Nat.add_comm m])]
+  . simp only [lift]
+    rw [if_neg, if_neg, Nat.add_assoc, Nat.add_comm j, ← Nat.add_assoc]
+    apply not_lt_of_le ((le_of_not_lt h₁).trans (Nat.le_add_right m k))
+    apply not_lt_of_le (by simpa [Nat.add_comm j] using h₃)
+| .sort _ => by simp
+| .app _ _ => by simp [lift_lift_of_le _ _ _ _ h]
+| .abs M N => by
+  simp [lift_lift_of_le _ _ _ _ h, Nat.add_assoc j n 1,
+        lift_lift_of_le _ _ _ _ (Nat.succ_le_succ h)]
+| .pi _ _ => by
+  simp [lift_lift_of_le _ _ _ _ h, Nat.add_assoc j n 1,
+        lift_lift_of_le _ _ _ _ (Nat.succ_le_succ h)]
 
-def lift_lift_of_le_of_le (i j k n : ℕ) :
-    i ≤ n → k ≤ i + n → ((M ↑ n # i) ↑ j # k) = M ↑ (n + j) # i := by
-  sorry
+lemma lift_lift_of_le_of_le (i j k n : ℕ) (h₁ : i ≤ k) (h₂ : k ≤ i + n) :
+  ∀ {M : PTerm S}, ((M ↑ n # i) ↑ j # k) = M ↑ (n + j) # i
+| .var m => by
+  simp only [lift]
+  split_ifs with h₃
+  . simp only [lift, if_pos (lt_of_lt_of_le h₃ h₁)]
+  . simp only [lift]
+    rw [if_neg, ← Nat.add_assoc]
+    apply not_lt_of_le (h₂.trans (Nat.add_le_add_right (le_of_not_lt h₃) _))
+| .sort _ => by simp
+| .app _ _ => by simp [lift_lift_of_le_of_le _ _ _ _ h₁ h₂]
+| .abs M N => by
+  simp [lift]
+  constructor
+  . rw [lift_lift_of_le_of_le _ _ _ _ h₁ h₂]
+  . rw [lift_lift_of_le_of_le _ _ _ _ (Nat.succ_le_succ h₁)]
+    rw [Nat.succ_add]; exact Nat.succ_le_succ h₂
+| .pi _ _ => by
+  simp [lift]
+  constructor
+  . rw [lift_lift_of_le_of_le _ _ _ _ h₁ h₂]
+  . rw [lift_lift_of_le_of_le _ _ _ _ (Nat.succ_le_succ h₁)]
+    rw [Nat.succ_add]; exact Nat.succ_le_succ h₂
 
-def lift0_lift0 (i j : ℕ) :
+lemma lift0_lift0 (i j : ℕ) :
     ((M ↑ i) ↑ j) = M ↑ (i + j) :=
   lift_lift_of_le_of_le _ _ _ _ (by simp) (by simp)
 
@@ -121,24 +168,145 @@ notation N "{" e " // " m "}" => subst e m N
 notation N "{" e "}" => subst e 0 N
 
 def subst_lift (i j k : ℕ) :
-    (M{N // j} ↑ k # (j + i)) = (M ↑ k # j + i + 1){N ↑ k # i // j} := by
-  sorry
+  ∀ {M N : PTerm S}, (M{N // j} ↑ k # (j + i)) = (M ↑ k # j + i + 1){N ↑ k # i // j}
+| .var m, N => by
+  simp; split_ifs with h₁ h₂ h₃ h₄ h₅
+  . simp; rw [if_pos (lt_of_lt_of_le h₁ (Nat.le_add_right _ _)), if_pos h₁]
+  . simpa using (not_lt_of_le $ (Nat.le_add_right j i).trans (Nat.le_add_right _ 1))
+      (lt_of_le_of_lt (le_of_not_lt h₂) h₁)
+  . simp [h₃]; rw [lift_lift_of_le _ _ _ _ (by simp)]
+  . simp [h₃] at h₄
+    simpa using (not_le_of_lt $ lt_of_le_of_lt (Nat.le_add_right j i) (Nat.lt_add_one _)) h₄
+  . simp
+    rw [if_pos, if_neg h₁, if_neg h₃]
+    rwa [Nat.sub_lt_iff_lt_add, Nat.add_comm 1]
+    apply Nat.one_le_of_lt $ lt_of_le_of_ne (le_of_not_lt h₁) (Ne.symm h₃)
+  . simp
+    have : j < m :=
+      lt_of_le_of_ne (le_of_not_lt h₁) (by simpa [eq_comm] using h₃)
+    rw [if_neg, if_neg, if_neg, Nat.sub_add_comm]
+    . apply Nat.one_le_of_lt $ lt_of_le_of_ne (le_of_not_lt h₁) (by simpa [eq_comm] using h₃)
+    . contrapose! this
+      simp [← this]
+    . contrapose! this
+      apply (Nat.le_add_right _ _).trans this.le
+    . simp; apply Nat.le_sub_of_add_le (le_of_not_lt h₅)
+| .sort _, _ => rfl
+| .app _ _, _ => by simp [subst_lift, subst_lift]
+| .abs _ _, _ => by
+  simp; constructor
+  . rw [subst_lift]
+  . rw [Nat.add_assoc j, Nat.add_comm i 1, ← Nat.add_assoc, subst_lift]
+| .pi _ _, _ => by
+  simp; constructor
+  . rw [subst_lift]
+  . rw [Nat.add_assoc j, Nat.add_comm i 1, ← Nat.add_assoc, subst_lift]
 
-def subst_lift_of_le (i j n : ℕ) :
-    i ≤ n → (M{N // n} ↑ j # i) = (M ↑ j # i){N // j + n} := by
-  sorry
+def subst_lift_of_le (i j n : ℕ) (h : i ≤ n) :
+  ∀ {M N : PTerm S}, (M{N // n} ↑ j # i) = (M ↑ j # i){N // j + n}
+| .var m, N => by
+  simp; split_ifs with h₁ h₂ h₃ h₄ h₅
+  . simp; rw [if_pos h₂, if_pos (Nat.lt_add_left _ h₁)]
+  . simp; rw [if_neg h₂, if_pos (by simpa [Nat.add_comm j])]
+  . rw [h₃] at h₄; simpa using not_le_of_lt h₄ h
+  . simp; rw [if_neg (by simp [h₃, Nat.add_comm]), if_pos (by rw [h₃, Nat.add_comm])]
+    rw [lift_lift_of_le_of_le _ _ _ _ (by simp) (by simpa [h₃])]
+  . simpa using lt_of_lt_of_le h₅ $ h.trans (le_of_not_lt h₁)
+  . simp
+    rw [if_neg, if_neg, if_neg, Nat.sub_add_comm]
+    . apply Nat.one_le_of_lt $ lt_of_le_of_ne (le_of_not_lt h₁) (Ne.symm h₃)
+    . contrapose! h₃
+      rw [Nat.add_comm, Nat.add_left_cancel_iff] at h₃
+      exact h₃
+    . contrapose! h₁
+      rw [Nat.add_comm, Nat.add_lt_add_iff_left] at h₁
+      exact h₁
+    . simp; apply Nat.le_sub_one_of_lt $ lt_of_le_of_lt h $
+        lt_of_le_of_ne (le_of_not_lt h₁) (Ne.symm h₃)
+| .sort _, _ => rfl
+| .app _ _, _ => by simp [subst_lift_of_le _ _ _ h]
+| .abs _ _, _ => by
+  simp; constructor
+  . rw [subst_lift_of_le _ _ _ h]
+  . rw [subst_lift_of_le _ _ _ (by simpa [Nat.add_le_add_iff_right]), ← Nat.add_assoc]
+| .pi _ _, _ => by
+  simp; constructor
+  . rw [subst_lift_of_le _ _ _ h]
+  . rw [subst_lift_of_le _ _ _ (by simpa [Nat.add_le_add_iff_right]), ← Nat.add_assoc]
 
-def lift_subst_of_le_of_le (i j k : ℕ) :
-    i ≤ k → k ≤ i + n → (M ↑ (n + 1) # j){N // k} = M ↑ n # i := by
-  sorry
+def lift_subst_of_le_of_le (i k n : ℕ) (h₁ : i ≤ k) (h₂ : k ≤ i + n) :
+    ∀ {M N : PTerm S}, (M ↑ (n + 1) # i){N // k} = M ↑ n # i
+| .var m, N => by
+  simp; split_ifs with h₃
+  . simp only [subst]; rw [if_pos (lt_of_lt_of_le h₃ h₁)]
+  . simp; rw [if_neg, if_neg]
+    . contrapose! h₂
+      rw [← h₂, Nat.add_comm n, ← Nat.add_assoc, Nat.add_lt_add_iff_right,
+          Nat.lt_add_one_iff]
+      exact le_of_not_lt h₃
+    . contrapose! h₂
+      exact (Nat.add_le_add (le_of_not_lt h₃) (Nat.le_add_right _ 1)).trans h₂
+| .sort _, _ => rfl
+| .app _ _, _ => by simp [lift_subst_of_le_of_le _ _ _ h₁ h₂]
+| .abs _ _, _ => by
+  simp; constructor
+  . rw [lift_subst_of_le_of_le _ _ _ h₁ h₂]
+  . rw [lift_subst_of_le_of_le _ _ _ (Nat.succ_le_succ h₁)]
+    rwa [Nat.succ_eq_add_one, Nat.succ_eq_add_one, Nat.add_assoc, Nat.add_comm 1,
+         ← Nat.add_assoc, Nat.add_le_add_iff_right]
+| .pi _ _, _ => by
+  simp; constructor
+  . rw [lift_subst_of_le_of_le _ _ _ h₁ h₂]
+  . rw [lift_subst_of_le_of_le _ _ _ (Nat.succ_le_succ h₁)]
+    rwa [Nat.succ_eq_add_one, Nat.succ_eq_add_one, Nat.add_assoc, Nat.add_comm 1,
+         ← Nat.add_assoc, Nat.add_le_add_iff_right]
 
 variable {P : PTerm S}
 
 def subst_subst (i j : ℕ) :
-    M{N // j}{P // i + j} = M{P // i + j + 1}{N{P // i} // j} := by
-  sorry
+    ∀ {M N : PTerm S}, M{N // j}{P // i + j} = M{P // i + j + 1}{N{P // i} // j}
+| .var n, N => by
+  simp; split_ifs with h₁ h₂ h₃ h₄ h₅ h₆ h₇ h₈
+  . simp; rw [if_pos (lt_of_lt_of_le h₁ (Nat.le_add_left _ _)), if_pos h₁]
+  . rw [h₃, Nat.add_assoc, Nat.add_comm j, ← Nat.add_assoc] at h₁
+    simpa using not_lt_of_le (Nat.le_add_left j (i + 1)) h₁
+  . have := (lt_of_le_of_ne (le_of_not_lt h₂) (Ne.symm h₃)).trans h₁
+    rw [Nat.add_assoc, Nat.add_comm j, ← Nat.add_assoc] at this
+    simpa using not_lt_of_le (Nat.le_add_left j (i + 1)) this
+  . simp [h₄]; rw [subst_lift_of_le _ _ _ (by simp), Nat.add_comm i]
+  . rw [h₄, Nat.add_assoc, Nat.add_comm j, ← Nat.add_assoc,
+      Nat.self_eq_add_left] at h₆
+    simpa using Nat.add_one_ne_zero _ h₆
+  . rw [h₄, Nat.add_comm i] at h₅
+    simpa using h₅ $ Nat.lt_add_one_of_le (Nat.le_add_right j i)
+  . simp
+    rw [if_pos, if_neg h₁, if_neg h₄]
+    rwa [Nat.sub_lt_iff_lt_add, Nat.add_comm]
+    apply Nat.one_le_of_lt $ lt_of_le_of_ne (le_of_not_lt h₁) (Ne.symm h₄)
+  . simp [h₈]; rw [lift_subst_of_le_of_le _ _ _ (by simp) (by simp)]
+  . simp
+    have aux₁ := lt_of_le_of_ne (le_of_not_lt h₇) (Ne.symm h₈)
+    have aux₂ := lt_of_le_of_ne (le_of_not_lt h₁) (Ne.symm h₄)
+    rw [if_neg, if_neg, if_neg, if_neg]
+    . contrapose! aux₁
+      rw [← aux₁, Nat.add_assoc, Nat.sub_add_cancel (Nat.one_le_of_lt aux₂)]
+      simp only [Nat.le_add_left]
+    . apply not_lt_of_le $ Nat.le_sub_one_of_lt aux₂
+    . contrapose! aux₁
+      rw [← aux₁, Nat.sub_add_cancel (Nat.one_le_of_lt aux₂)]
+    . apply not_lt_of_le $ Nat.le_sub_one_of_lt (lt_trans (Nat.lt_add_one _) aux₁)
+| .sort _, _ => rfl
+| .app _ _, _ => by simp [subst_subst]
+| .abs _ _, _ => by
+  simp; constructor
+  . rw [subst_subst]
+  . rw [Nat.add_assoc i, subst_subst]
+| .pi _ _, _ => by
+  simp; constructor
+  . rw [subst_subst]
+  . rw [Nat.add_assoc i, subst_subst]
 
-def subst0_subst0 (k : ℕ) :
+def subst0_subst (k : ℕ) :
     M{N}{P // k} = M{P // k + 1}{N{P // k}} :=
   subst_subst _ 0
 
@@ -152,11 +320,15 @@ def PCtx.lift (i c : ℕ) : PCtx S → PCtx S := List.map (PureTypeSystem.lift i
 
 notation Γ" ↑↑ "i" # "c => PCtx.lift i c Γ
 
+@[simp]
+lemma PCtx.lift_length {i c : ℕ} {Γ : PCtx S} : (Γ ↑↑ i # c).length = Γ.length :=
+  List.length_map _ _
+
 notation Γ" ↑↑ "i => PCtx.lift i 0 Γ
 
 variable {α : Type*}
 
-inductive isItem : α → List α → ℕ → Prop
+inductive isItem : α → List α → ℕ → Type _
 | zero Γ : isItem x (x :: Γ) 0
 | succ {Γ n} y : isItem x Γ n → isItem x (y :: Γ) (n + 1)
 
@@ -166,9 +338,7 @@ lemma isItem.lt_length : ∀ (_ : x ↓ n in Γ), n < length Γ
 | .zero _ => by simp
 | .succ x h => by simp; apply lt_length h
 
--- need a better name
-
-def isItem_unique {x y : α} {Γ : List α} {n : ℕ} :
+lemma isItem_unique {x y : α} {Γ : List α} {n : ℕ} :
     (x ↓ n in Γ) → (y ↓ n in Γ) → x = y := by
   induction n generalizing x y Γ
   . intro h₁ h₂
@@ -177,6 +347,12 @@ def isItem_unique {x y : α} {Γ : List α} {n : ℕ} :
     cases h₁; cases h₂
     rename_i ih _ _ h₁ h₂
     apply ih h₁ h₂
+
+def isItem.pred {x y : α} {Γ : List α}: ∀ (_ : x ↓ (n + 1) in (y :: Γ)), x ↓ n in Γ
+| .succ _ h => h
+
+lemma isItem.eq {x y : α} {Γ : List α} : ∀ (_ : x ↓ 0 in y :: Γ), x = y
+| .zero _ => rfl
 
 -- isTruncate the first k-term and have =
 inductive isTrunc : ℕ → List α → List α → Type _
@@ -187,9 +363,9 @@ def isTrunc.pred : ∀ {k Γ Δ} {A : PTerm S} (_ : isTrunc k Γ (A :: Δ)), isT
 | 0, _, _, _, h => by cases h; apply isTrunc.succ; apply isTrunc.zero
 | k, [], Δ, A, h => by cases h
 | k + 1, B :: Γ, Δ, A, h => by
-    apply isTrunc.succ
-    cases h
-    apply isTrunc.pred (by assumption)
+  apply isTrunc.succ
+  cases h
+  apply isTrunc.pred (by assumption)
 
 def isTrunc.nil_length {Γ : List α}: ∀ {k} (_ : isTrunc k Γ []), Γ.length = k
 | 0, h => by cases h; rfl
@@ -213,21 +389,23 @@ lemma isTrunc.heads_length : ∀  {k : ℕ} {Γ Δ : List α} (h : isTrunc k Γ 
 | k + 1, A :: Γ, Δ, .succ _ h => by
   simpa [heads] using h.heads_length
 
-/-
-def exist_isTrunc_of_isItem (k : ℕ) (Γ : List α) (x : α) :
-    (x ↓ k in Γ) → ∃ Γ', isTrunc (k + 1) Γ Γ' := by
-  induction k generalizing x Γ
-  . intro h; cases h; rename_i Γ
-    exact ⟨Γ, isTrunc.succ _ (isTrunc.zero _)⟩
-  . intro h; cases h
-    rename_i ih _ _ h
-    obtain ⟨Γ', hΓ'⟩ := ih _ _ h
-    exact ⟨Γ', isTrunc.succ _ hΓ'⟩
--/
-def isIerm_of_isTrunc {Γ Δ : List α} {A : α} : ∀ {k : ℕ},
+def isTrunc.isItem {Γ Δ : List α} {A : α} : ∀ {k : ℕ},
     isTrunc k Γ (A :: Δ) → A ↓ k in Γ
 | 0, h => by cases h; apply isItem.zero
-| k + 1, .succ _ h => isItem.succ _ (isIerm_of_isTrunc h)
+| k + 1, .succ _ h => isItem.succ _ h.isItem
+
+def isItem.isTrunc {k : ℕ} {Γ : List α} {x : α} :
+  (_ : x ↓ k in Γ) → Σ Γ', isTrunc (k + 1) Γ Γ'
+| .zero Γ => ⟨Γ, isTrunc.succ _ (isTrunc.zero _)⟩
+| .succ y h => by
+  exact ⟨_, isTrunc.succ _ h.isTrunc.2⟩
+
+lemma exists_isTrunc_of_isItem {k : ℕ} {Γ : List α} {x : α} :
+  (_ : x ↓ k in Γ) → ∃ Γ', Nonempty (isTrunc (k + 1) Γ Γ')
+| .zero Γ => ⟨Γ, ⟨isTrunc.succ _ (isTrunc.zero _)⟩⟩
+| .succ y h => by
+  obtain ⟨Γ, ⟨hΓ⟩⟩ := exists_isTrunc_of_isItem h
+  exact ⟨Γ, ⟨isTrunc.succ _ hΓ⟩⟩
 
 inductive isInsert (Γ : PCtx S) (t : PTerm S) : ℕ → PCtx S → PCtx S → Type _
 | zero : isInsert Γ t 0 Γ (t :: Γ)
@@ -249,48 +427,86 @@ def isItem_of_isInsert_of_le {t : PTerm S} {n : ℕ} {Γ Δ Δ' : PCtx S} :
       simp at hk
       apply ih ht hk hu
 
-def isItem_of_isInsert_of_lt {t : PTerm S} {n : ℕ} {Γ Δ Δ' : PCtx S} :
-    isInsert Γ t n Δ Δ' → ∀ {k}, (k < n → ∀ {u}, (u ↓ k in Δ) →
-      (u ↑ 1 # (n - (k + 1)) ) ↓ k in Δ') := by
-  sorry
+def isItem_of_isInsert_of_lt {u t : PTerm S} {n k : ℕ} {Γ Δ Δ' : PCtx S} :
+    isInsert Γ t n Δ Δ' → k < n → (u ↓ k in Δ) → (u ↑ 1 # (n - (k + 1)) ) ↓ k in Δ'
+| .zero, h, _ => by simp at h
+| .succ _ h₁, h₂, .zero _ => by simpa using isItem.zero _
+| .succ _ h₁, h₂, .succ _ h₃ => by
+  simpa using isItem.succ _ (isItem_of_isInsert_of_lt h₁ (by simpa using h₂) h₃)
 
-def isItemLift (t : PTerm S) (Γ : PCtx S) (n : ℕ) : Prop :=
-    ∃ u, (t = u ↑ n + 1) ∧ u ↓ n in Γ
+structure isItemLift (t : PTerm S) (Γ : PCtx S) (n : ℕ) where
+  item : PTerm S
+  eq : t = item ↑ n + 1
+  is : item ↓ n in Γ
 
 notation x " ↓ " n " sub " Γ => isItemLift x Γ n
+
+lemma isItemLift.eq_lift_one {t u : PTerm S} {Γ : PCtx S} (h : t ↓ 0 sub (u :: Γ)) :
+    t = u ↑ 1 := by
+  simp only [h.2, h.3.eq]
 
 def isItemLift_of_isInsert_of_lt {t u : PTerm S} {n : ℕ} {Γ Δ Δ' : PCtx S}
   (h : isInsert Γ t n Δ Δ') {k : ℕ} (hk : k < n) (hu : u ↓ k sub Δ) :
     (u ↑ 1 # n) ↓ k sub Δ' := by
-  rcases hu with ⟨w, ⟨hw₁, hw₂⟩⟩
-  use w ↑ 1 # (n - (k + 1))
-  constructor
-  . rw [hw₁]
-    have : n = (k + 1) + (n - (k + 1)) :=  (Nat.add_sub_of_le hk).symm
-    rw [this, lift_lift_of_le _ _ _ _ (Nat.zero_le _)]
-    congr
-  . clear u hw₁
-    cases h
-    . simp at hk
-    . rename_i n Δ Δ' u ht
-      cases hw₂
-      . apply isItem.zero
-      . rename_i n' hw
-        apply isItem.succ
-        simp at hk ⊢
-        apply isItem_of_isInsert_of_lt ht hk hw
+  cases hu with
+  | mk w hw₁ hw₂ =>
+    use w ↑ 1 # (n - (k + 1))
+    . rw [hw₁]
+      have : n = (k + 1) + (n - (k + 1)) :=  (Nat.add_sub_of_le hk).symm
+      rw [this, lift_lift_of_le _ _ _ _ (Nat.zero_le _)]
+      congr
+    . clear u hw₁
+      cases h
+      . simp at hk
+      . rename_i n Δ Δ' u ht
+        cases hw₂
+        . apply isItem.zero
+        . rename_i n' hw
+          apply isItem.succ
+          simp at hk ⊢
+          apply isItem_of_isInsert_of_lt ht hk hw
 
 inductive isSubst (Γ : PCtx S) (t T : PTerm S) : ℕ → PCtx S → PCtx S → Type _
 | zero : isSubst Γ t T 0 (T :: Γ) Γ
 | succ {n Δ Δ'} w : isSubst Γ t T n Δ Δ' → isSubst Γ t T (n + 1) (w :: Δ) (w{t // n} :: Δ')
 
-def isTerm_of_isSubst_of_le {n : ℕ} {Γ Δ Δ' : PCtx S} {t T : PTerm S} :
-    isSubst Γ t T n Δ Δ' → ∀ {k}, n ≤ k → (∀ {v}, (v ↓ k + 1 in Δ) → v ↓ k in Δ') := by
-  induction n
-  . intro h k hk v hv
-    cases h; cases hv
-    assumption
-  . sorry
+def isItem_of_isSubst_of_le {Γ Δ Δ' : PCtx S} {a A B : PTerm S} {n : ℕ} :
+    {k : ℕ} → isSubst Γ a A n Δ Δ' → n ≤ k → (B ↓ k + 1 in Δ) → B ↓ k in Δ'
+| _, .zero, _, .succ _ h => h
+| k + 1, .succ _ h₁, h₂, .succ _ h₃ => by
+  apply isItem.succ
+  apply isItem_of_isSubst_of_le h₁ (by simpa using h₂) h₃
+
+
+def isItem_of_isSubst_of_lt {Γ Δ Δ' : PCtx S} {a A B : PTerm S} {n k : ℕ} :
+    isSubst Γ a A n Δ Δ' → k < n → (B ↓ k in Δ) → B{a // n - (k + 1)} ↓ k in Δ'
+| .zero, h, _ => by simp at h
+| .succ _ h₁, h₂, .zero _ => by
+  simp; apply isItem.zero
+| .succ _ h₁, h₂, .succ _ h₃ => by
+  apply isItem.succ
+  simp
+  apply isItem_of_isSubst_of_lt h₁ (by simpa using h₂) h₃
+
+def isItemLift_of_isSubst_of_lt {Γ Δ Δ' : PCtx S} {a A B : PTerm S} {n k : ℕ} :
+    isSubst Γ a A n Δ Δ' → k < n → (B ↓ k sub Δ) → B{a // n} ↓ k sub Δ' := by
+  intro h₁ h₂ h₃
+  use h₃.1{a // n - (k + 1)}
+  . conv_lhs => rw [h₃.2]
+    rw [subst_lift_of_le _ _ _ (by simp)]
+    congr 1
+    rw [Nat.add_sub_cancel' (by simpa)]
+  . apply isItem_of_isSubst_of_lt h₁ h₂ h₃.3
+
+lemma eq_of_isSubst_of_isItem {n : ℕ} {Γ Δ Δ' : PCtx S} {a A B: PTerm S} :
+    isSubst Γ a A n Δ Δ' → (B ↓ n in Δ) → A = B
+| .zero, h => by cases h; rfl
+| .succ _ h₁, .succ _ h₂ => eq_of_isSubst_of_isItem h₁ h₂
+
+def isSubst.isTrunc {n : ℕ} {Γ Δ Δ' : PCtx S} {a A : PTerm S} :
+    isSubst Γ a A n Δ Δ' → isTrunc n Δ' Γ
+| .zero => isTrunc.zero _
+| .succ _ h => isTrunc.succ _ h.isTrunc
 
 end Context
 
@@ -325,17 +541,32 @@ infix:50 " ≃β " => betac
 
 def betac.refl (A : PTerm S) : A ≃β A := betac.betar _ _ (betar.refl _)
 
-def beta.lift (h : A →β B) :
-    (A ↑ i # n) →β B ↑ i # n := by
-  sorry
+def beta.betac {A B : PTerm S} (h : A →β B) : A ≃β B := betac.betar _ _ (betar.beta _ _ h)
 
-def betar.lift (h : A ↠β B) :
-    (A ↑ i # n) ↠β B ↑ i # n := by
-  sorry
+def betar.betac {A B : PTerm S} (h : A ↠β B) : A ≃β B := betac.betar _ _ h
 
-def betac.lift (h : A ≃β B) :
-    (A ↑ i # n) ≃β B ↑ i # n := by
-  sorry
+def beta.lift : (h : A →β B) → (A ↑ i # n) →β B ↑ i # n
+| .red A M N => by
+  have : n = 0 + n := by simp
+  conv_rhs =>
+    rw [this, subst_lift]
+  simpa using beta.red _ _ _
+| .appl _ _ _ h => by simpa using beta.appl _ _ _ (beta.lift h)
+| .appr _ _ _ h => by simpa using beta.appr _ _ _ (beta.lift h)
+| .pil _ _ _ h => by simpa using beta.pil _ _ _ (beta.lift h)
+| .pir _ _ _ h => by simpa using beta.pir _ _ _ (beta.lift h)
+| .absl _ _ _ h => by simpa using beta.absl _ _ _ (beta.lift h)
+| .absr _ _ _ h => by simpa using beta.absr _ _ _ (beta.lift h)
+
+def betar.lift : (h : A ↠β B) → (A ↑ i # n) ↠β B ↑ i # n
+| .beta _ _ h => betar.beta _ _ h.lift
+| .refl _ => betar.refl _
+| .trans _ _ _ h₁ h₂ => h₁.lift.trans _ _ _ h₂.lift
+
+def betac.lift : (h : A ≃β B) → (A ↑ i # n) ≃β B ↑ i # n
+| .betar _ _ h => betac.betar _ _ h.lift
+| .symm _ _ h => h.lift.symm
+| .trans _ _ _ h₁ h₂ => h₁.lift.trans _ _ _ h₂.lift
 
 def betar.appl {A A' B : PTerm S} : ∀ (_ : A ↠β A'), A ⬝ B ↠β A' ⬝ B
 | .beta _ _ h => beta _ _ (beta.appl _ _ _ h)
@@ -423,7 +654,7 @@ def betac.pi  {A B A' B' : PTerm S} (h₁ : A ≃β A') (h₂ : B ≃β B') :
 
 def beta.substl {A B C : PTerm S} {n : ℕ} : ∀ (_ : A →β B), A{C//n} →β B{C//n}
 | .red A M N => by
-  simpa [subst0_subst0] using beta.red (A{C // n}) (M{C // n + 1}) (N{C // n})
+  simpa [subst0_subst] using beta.red (A{C // n}) (M{C // n + 1}) (N{C // n})
 | .appl _ _ _ h => h.substl.appl _ _ _
 | .appr _ _ _ h => h.substl.appr _ _ _
 | .absl _ _ _ h => h.substl.absl _ _ _
@@ -473,11 +704,227 @@ def betac.subst {A A' B B' : PTerm S} {n : ℕ} (h₁ : A ≃β A') (h₂ : B �
     A{B // n} ≃β A'{B'//n} :=
   h₁.substl.trans _ _ _ h₂.substr
 
-lemma betar.eq_of_sort_betar {s : S.sort} {A : PTerm S} :
-    (!s) ↠β A → A = !s := sorry
+lemma betar.eq_of_sort_betar' {s : S.sort} {A B : PTerm S} (h : B = !s):
+    B ↠β A → A = !s
+| .beta _ _ h' => by cases h; cases h'
+| .refl _ => h
+| .trans _ _ _ h₁ h₂ => h₂.eq_of_sort_betar' (h₁.eq_of_sort_betar' h)
 
-def betac.confl {A B : PTerm S} (h : A ≃β B) : Σ (C : PTerm S), (A ↠β C) × (B ↠β C) := sorry
+lemma betar.eq_of_sort_betar {s : S.sort} {A : PTerm S} :
+    (!s) ↠β A → A = !s
+| h => h.eq_of_sort_betar' rfl
+
+lemma betar.eq_of_var_betar' {n : ℕ} {A B : PTerm S} (h : B = #n):
+    B ↠β A → A = #n
+| .beta _ _ h' => by cases h; cases h'
+| .refl _ => h
+| .trans _ _ _ h₁ h₂ => h₂.eq_of_var_betar' (h₁.eq_of_var_betar' h)
+
+lemma betar.eq_of_var_betar {n : ℕ} {A : PTerm S} :
+    (#n) ↠β A → A = #n
+| h => h.eq_of_var_betar' rfl
+
+structure betar.PiStruct (A B C : PTerm S) where
+  left : PTerm S
+  right : PTerm S
+  eq : C = Π.left right
+  betarl : A ↠β left
+  betarr : B ↠β right
+
+def betar.PiStruct.trans {A B A' B' C C' : PTerm S} (S : PiStruct A B C)
+  (h₁ : A' = S.left) (h₂ : B' = S.right) (S' : PiStruct A' B' C') :
+    PiStruct A B C' where
+  left := S'.left
+  right := S'.right
+  eq := S'.eq
+  betarl := by
+    cases h₁
+    exact S.betarl.trans _ _ _ S'.betarl
+  betarr := by
+    cases h₂
+    exact S.betarr.trans _ _ _ S'.betarr
+
+def beta.of_pi_beta {A B C : PTerm S} :
+    (h : Π.A B →β C) → betar.PiStruct A B C
+| .pil _ A' _ h => ⟨A', _, rfl, betar.beta _ _ h, betar.refl _⟩
+| .pir _ _ B' h => ⟨_, B', rfl, betar.refl _, betar.beta _ _ h⟩
+
+def betar.of_pi_betar' {A B C D : PTerm S} (h : D = Π.A B) :
+    (h : D ↠β C) → PiStruct A B C
+| .beta _ _ h' => by cases h; exact h'.of_pi_beta
+| .refl _ => by cases h; exact ⟨_, _, rfl, betar.refl _, betar.refl _⟩
+| .trans _ _ _ h₁ h₂ =>
+  (h₁.of_pi_betar' h).trans rfl rfl (h₂.of_pi_betar' (h₁.of_pi_betar' h).eq)
+
+def betar.of_pi_betar {A B C : PTerm S} (h : Π.A B ↠β C) :
+    PiStruct A B C := h.of_pi_betar' rfl
+
+section Confluence
+/--
+  Parallel reduction
+-/
+inductive betap : PTerm S → PTerm S → Type _
+| var n : betap (#n) (#n)
+| sort s : betap (!s) (!s)
+| pi A A' M M' : betap A A' → betap M M' → betap (Π.A M) (Π.A' M')
+| abs A A' M M' : betap A A' → betap M M' → betap (λ.A M) (λ.A' M')
+| app A A' M M' : betap A A' → betap M M' → betap (A ⬝ M) (A' ⬝ M')
+| red A M M' N N' : betap M M' → betap N N' → betap ((λ. A M) ⬝ N) (M'{N'})
+
+inductive betapr : PTerm S → PTerm S → Type _
+| betap x y : betap x y → betapr x y
+| refl x : betapr x x
+| trans x y z : betapr x y → betapr y z → betapr x z
+
+infix:50 " →'β " => betap
+
+infix:50 " ↠'β " => betapr
+
+def betap.refl : (A : PTerm S) → A →'β A
+| .var _ => var _
+| .sort _ => sort _
+| .app _ _ => app _ _ _ _ (refl _) (refl _)
+| .abs _ _ => abs _ _ _ _ (refl _) (refl _)
+| .pi _ _ => pi _ _ _ _ (refl _) (refl _)
+
+def betap.lift {i c : ℕ} {A B : PTerm S} : A →'β B → (A ↑ i # c) →'β (B ↑ i # c)
+| .var _ => by
+  simp; split_ifs
+  <;> apply var
+| .sort _ => betap.sort _
+| .app _ _ _ _ h₁ h₂ => app _ _ _ _ h₁.lift h₂.lift
+| .abs _ _ _ _ h₁ h₂ => abs _ _ _ _ h₁.lift h₂.lift
+| .pi _ _ _ _ h₁ h₂ => pi _ _ _ _ h₁.lift h₂.lift
+| .red _ _ _ _ _ h₁ h₂ => by
+  have : c = 0 + c := by simp
+  conv_rhs => rw [this, subst_lift]; simp
+  apply red _ _ _ _ _ h₁.lift h₂.lift
+
+def betap.subst {n : ℕ} {A B : PTerm S} :
+  A →'β A' → B →'β B' → A{B // n} →'β A'{B'// n}
+| .var _, h => by
+  simp; split_ifs
+  . apply var
+  . apply h.lift
+  . apply var
+| .sort _, _ => betap.sort _
+| .app _ _ _ _ h₁ h₂, h => app _ _ _ _ (h₁.subst h) (h₂.subst h)
+| .abs _ _ _ _ h₁ h₂, h => abs _ _ _ _ (h₁.subst h) (h₂.subst h)
+| .pi _ _ _ _ h₁ h₂, h => pi _ _ _ _ (h₁.subst h) (h₂.subst h)
+| .red _ _ _ _ _ h₁ h₂, h => by
+  simp
+  have : n = n + 0 := rfl
+  conv_rhs => rw [this, subst_subst n 0]; simp
+  apply red _ _ _ _ _ (h₁.subst h) (h₂.subst h)
+
+def betap.betar {A B : PTerm S} :
+    A →'β B → A ↠β B
+| .var _ => betar.refl _
+| .sort _ => betar.refl _
+| .app _ _ _ _ h₁ h₂ => betar.app h₁.betar h₂.betar
+| .abs _ _ _ _ h₁ h₂ => betar.abs h₁.betar h₂.betar
+| .pi _ _ _ _ h₁ h₂ => betar.pi h₁.betar h₂.betar
+| .red _ _ _ _ _ h₁ h₂ =>
+  betar.trans _ _ _ (betar.beta _ _ (beta.red _ _ _))
+    (betar.subst (h₁ := h₁.betar) (h₂ := h₂.betar))
+
+def betapr.betar {A B : PTerm S} :
+    A ↠'β B → A ↠β B
+| .betap _ _ h => h.betar
+| .refl _ => betar.refl _
+| .trans _ _ _ h₁ h₂ => h₁.betar.trans _ _ _ h₂.betar
+
+def beta.betap {A B : PTerm S} :
+    A →β B → A →'β B
+| .red _ _ _ => betap.red _ _ _ _ _ (betap.refl _) (betap.refl _)
+| .appl _ _ _ h => betap.app _ _ _ _ h.betap (betap.refl _)
+| .appr _ _ _ h => betap.app _ _ _ _ (betap.refl _) h.betap
+| .pil _ _ _ h => betap.pi _ _ _ _ h.betap (betap.refl _)
+| .pir _ _ _ h => betap.pi _ _ _ _ (betap.refl _) h.betap
+| .absl _ _ _ h => betap.abs _ _ _ _ h.betap (betap.refl _)
+| .absr _ _ _ h => betap.abs _ _ _ _ (betap.refl _) h.betap
+
+def beta.betapr {A B : PTerm S} :
+    A →β B → A ↠'β B :=
+  fun h ↦ betapr.betap _ _ h.betap
+
+def betar.betapr {A B : PTerm S} :
+    A ↠β B → A ↠'β B
+| .beta _ _ h => h.betapr
+| .refl _ => betapr.refl _
+| .trans _ _ _ h₁ h₂ => h₁.betapr.trans _ _ _ h₂.betapr
+
+def betap.diamond {A B C : PTerm S} :
+  A →'β B → A →'β C → Σ D, B →'β D × C →'β D
+| .var _, .var _ => ⟨_, refl _, refl _⟩
+| .sort _, .sort _ => ⟨_, refl _, refl _⟩
+| .pi _ _ _ _ h₁ h₂, .pi _ _ _ _ h₃ h₄ =>
+  ⟨_, pi _ _ _ _ (h₁.diamond h₃).2.1 (h₂.diamond h₄).2.1,
+    pi _ _ _ _ (h₁.diamond h₃).2.2 (h₂.diamond h₄).2.2⟩
+| .abs _ _ _ _ h₁ h₂, .abs _ _ _ _ h₃ h₄ =>
+  ⟨_, abs _ _ _ _ (h₁.diamond h₃).2.1 (h₂.diamond h₄).2.1,
+    abs _ _ _ _ (h₁.diamond h₃).2.2 (h₂.diamond h₄).2.2⟩
+| .app _ _ _ _ h₁ h₂, .app _ _ _ _ h₃ h₄ =>
+  ⟨_, app _ _ _ _ (h₁.diamond h₃).2.1 (h₂.diamond h₄).2.1,
+    app _ _ _ _ (h₁.diamond h₃).2.2 (h₂.diamond h₄).2.2⟩
+| .app _ _ _ _ (.abs _ _ _ _ _ h₁) h₂, .red _ _ _ _ _ h₃ h₄ =>
+  ⟨_, red _ _ _ _ _ (h₁.diamond h₃).2.1 (h₂.diamond h₄).2.1,
+    subst (h₁.diamond h₃).2.2 (h₂.diamond h₄).2.2⟩
+| .red _ _ _ _ _ h₁ h₂, .red _ _ _ _ _ h₃ h₄ =>
+  ⟨_, subst (h₁.diamond h₃).2.1 (h₂.diamond h₄).2.1,
+    subst (h₁.diamond h₃).2.2 (h₂.diamond h₄).2.2⟩
+| .red _ _ _ _ _ h₁ h₂, .app _ _ _ _ (.abs _ _ _ _ _ h₃) h₄ =>
+  ⟨_, subst (h₁.diamond h₃).2.1 (h₂.diamond h₄).2.1,
+    red _ _ _ _ _ (h₁.diamond h₃).2.2 (h₂.diamond h₄).2.2⟩
+
+def betap.diamond_aux {A B C : PTerm S} :
+  A →'β B → A ↠'β C → Σ D, B ↠'β D × C →'β D
+| h₁, .betap _ _ h₂ => ⟨_, betapr.betap _ _ (h₁.diamond h₂).2.1, (h₁.diamond h₂).2.2⟩
+| h₁, .refl _ => ⟨_, betapr.refl _, h₁⟩
+| h₁, .trans _ _ _ h₂ h₃ => by
+  let h₄ := h₁.diamond_aux h₂
+  exact ⟨_, h₄.2.1.trans _ _ _ (h₄.2.2.diamond_aux h₃).2.1,
+    (h₄.2.2.diamond_aux h₃).2.2⟩
+
+def betapr.diamond {A B C : PTerm S} :
+  A ↠'β B → A ↠'β C → Σ D, B ↠'β D × C ↠'β D
+| .betap _ _ h₁, h₂ => ⟨_, (h₁.diamond_aux h₂).2.1, betapr.betap _ _ (h₁.diamond_aux h₂).2.2⟩
+| .refl _, h₂ => ⟨_, h₂, betapr.refl _⟩
+| .trans _ _ _ h₁ h₂, h₃ => by
+  let h₄ := h₁.diamond h₃
+  exact ⟨_, (h₂.diamond h₄.2.1).2.1, h₄.2.2.trans _ _ _ (h₂.diamond h₄.2.1).2.2⟩
+
+def betar.diamond {A B C : PTerm S} :
+    A ↠β B → A ↠β C → Σ D, B ↠β D × C ↠β D :=
+  fun h₁ h₂ ↦ ⟨_, (h₁.betapr.diamond h₂.betapr).2.1.betar,
+    (h₁.betapr.diamond h₂.betapr).2.2.betar⟩
+
+def betac.confl {A B : PTerm S} :
+    A ≃β B → Σ (C : PTerm S), (A ↠β C) × (B ↠β C)
+| .betar _ _ h => ⟨_, h, betar.refl _⟩
+| .symm _ _ h => ⟨_, h.confl.2.2, h.confl.2.1⟩
+| .trans _ _ _ h₁ h₂ =>
+  ⟨_, h₁.confl.2.1.trans _ _ _ (h₁.confl.2.2.diamond h₂.confl.2.1).2.1,
+    h₂.confl.2.2.trans _ _ _ (h₁.confl.2.2.diamond h₂.confl.2.1).2.2⟩
+
 alias betac_confl := betac.confl
+
+end Confluence
+
+def betac_of_pi_betac {A B A' B' : PTerm S} (h : Π.A B ≃β Π.A' B') :
+    A ≃β A' × B ≃β B' := by
+  have := h.confl.2.1.of_pi_betar.eq.symm.trans h.confl.2.2.of_pi_betar.eq
+  simp only [pi.injEq] at this
+  constructor
+  . apply betac.trans
+    apply h.confl.2.1.of_pi_betar.betarl.betac
+    rw [this.1]
+    exact h.confl.2.2.of_pi_betar.betarl.betac.symm
+  . apply betac.trans
+    apply h.confl.2.1.of_pi_betar.betarr.betac
+    rw [this.2]
+    exact h.confl.2.2.of_pi_betar.betarr.betac.symm
+alias pi_inj := betac_of_pi_betac
 
 def betar_of_betac_sort {s : S.sort} {t : PTerm S} (h : t ≃β (!s)) :
     t ↠β (!s) := by
@@ -565,11 +1012,51 @@ def exists_of_sort_typing : ∀ (_ : Γ ⊢ !s : A),
     use C
     exact ⟨EqvGen.trans _ _ _ hC.1 h₀, hC.2⟩
 -/
-/-
-def exists_of_pi_typing : ∀ (_ : Γ ⊢ Π.A B : T),
-    ∃ s₁ s₂ s₃, (T ≃β !s₃) ∧ S.rel s₁ s₂ s₃ ∧ Nonempty (Γ ⊢ A : !s₁) ∧ Nonempty (A :: Γ ⊢ B : !s₂) :=
-  sorry
 
+lemma exists_of_pi_typing : ∀ (_ : Γ ⊢ Π.A B : T),
+    ∃ s₁ s₂ s₃, Nonempty (T ≃β !s₃) ∧ S.rel s₁ s₂ s₃ ∧
+      Nonempty (Γ ⊢ A : !s₁) ∧ Nonempty (A :: Γ ⊢ B : !s₂)
+| .pi _ _ _ s₁ s₂ s₃ h₁ h₂ h₃ => ⟨s₁, s₂, s₃, ⟨betac.refl _⟩, h₁, ⟨h₂⟩, ⟨h₃⟩⟩
+| .conv _ _ _ _ _ h₁ h₂ h₃ => by
+  obtain ⟨s₁, s₂, s₃, ⟨h₄⟩, h₅, ⟨h₆⟩, ⟨h₇⟩⟩ := exists_of_pi_typing h₂
+  exact ⟨s₁, s₂, s₃, ⟨⟨(h₁.symm).trans _ _ _ h₄⟩, h₅, ⟨h₆⟩, ⟨h₇⟩⟩⟩
+
+structure PiTypingStruct {Γ : PCtx S} {A B T : PTerm S} (h : Γ ⊢ Π.A B : T) where
+  s₁ : S.sort
+  s₂ : S.sort
+  s₃ : S.sort
+  betac : T ≃β !s₃
+  rel : S.rel s₁ s₂ s₃
+  typing₁ : Γ ⊢ A : !s₁
+  typing₂ : A :: Γ ⊢ B : !s₂
+
+def of_pi_typing : ∀ (h : Γ ⊢ Π.A B : T), PiTypingStruct h
+| .pi _ _ _ s₁ s₂ s₃ h₁ h₂ h₃ => ⟨s₁, s₂, s₃, betac.refl _, h₁, h₂, h₃⟩
+| .conv _ _ _ _ _ h₁ h₂ h₃ => by
+  exact ⟨_, _, _, (h₁.symm).trans _ _ _ (of_pi_typing h₂).betac,
+    (of_pi_typing h₂).rel, (of_pi_typing h₂).typing₁, (of_pi_typing h₂).typing₂⟩
+alias pi_inversion := of_pi_typing
+
+structure AbsTypingStruct {Γ : PCtx S} {A b T : PTerm S} (h : Γ ⊢ λ.A b : T) where
+  s₁ : S.sort
+  s₂ : S.sort
+  s₃ : S.sort
+  type : PTerm S
+  betac : T ≃β Π.A type
+  rel : S.rel s₁ s₂ s₃
+  typing₁ : Γ ⊢ A : !s₁
+  typing₂ : A :: Γ ⊢ type : !s₂
+  typing₃ : A :: Γ ⊢ b : type
+
+def of_abs_typing : ∀ (h : Γ ⊢ λ.A b : T), AbsTypingStruct h
+| .abs _ _ _ _ _ _ _ h₀ h₁ h₂ h₃ => ⟨_, _, _, _, betac.refl _, h₀, h₁, h₂, h₃⟩
+| .conv _ _ _ _ _ h₁ h₂ h₃ => by
+  exact ⟨_, _, _, _, (h₁.symm).trans _ _ _ (of_abs_typing h₂).betac,
+    (of_abs_typing h₂).rel, (of_abs_typing h₂).typing₁,
+    (of_abs_typing h₂).typing₂, (of_abs_typing h₂).typing₃⟩
+alias abs_inversion := of_pi_typing
+
+/-
 def exists_of_abs_typing (h : Derivable (Γ ⊢ λ.A b : T)) :
     ∃ s₁ s₂ s₃, ∃ B, (T ≃β Π.A B) ∧ S.rel s₁ s₂ s₃ ∧
       Derivable (Γ ⊢ A : !s₁) ∧ Derivable (A :: Γ ⊢ b : B) ∧
@@ -600,63 +1087,175 @@ def exists_of_app_typing (h : Derivable (Γ ⊢ f ⬝ a : T)) :
 -/
 
 mutual
-def weakening_typing : ∀ (_ : Γ ⊢ t : T) (_ : isInsert Δ A n Γ Γ') (_ : Δ ⊢ A : !s),
+def weakening_typing : (Γ ⊢ t : T) → isInsert Δ A n Γ Γ' → (Δ ⊢ A : !s) →
     (Γ' ⊢ t ↑ 1 # n : T ↑ 1 # n)
-| .var Γ A k h₀ h₁, h₂, h₃ => by
+| .var _ _ k h₀ h₁, h₂, h₃ => by
   dsimp
   split_ifs with h
-  . apply typing.var _ _ _ _
-      (isItemLift_of_isInsert_of_lt h₂ h h₁)
-    apply (weakening_wf h₀ h₂ h₃)
   . apply typing.var _ _ _ (weakening_wf h₀ h₂ h₃)
-    obtain ⟨T', hT'⟩ := h₁
-    use T'
-    rw [hT'.1]
-    constructor
+      (isItemLift_of_isInsert_of_lt h₂ h h₁)
+  . apply typing.var _ _ _ (weakening_wf h₀ h₂ h₃)
+    use h₁.1
+    conv_lhs => rw [h₁.2]
     . rw [lift_lift_of_le_of_le _ _ _ _ (by simp)
         (by simp at h ⊢; apply h.trans (Nat.le_succ _))]
-    . apply isItem_of_isInsert_of_le h₂ (by simpa using h) hT'.2
-| .sort Γ s₁ s₂ h₀ h₁, h₂, h₃ => by
-    simp; apply typing.sort _ _ _ h₀ (weakening_wf h₁ h₂ h₃)
-| .pi Γ A B s₁ s₂ s₃ h₀ h₁ h₃, h₄, h₅ => by
-  apply typing.pi
-  apply h₀
-  apply weakening_typing h₁ h₄ h₅
-  apply weakening_typing h₃ (h₄.succ A) h₅
-| .abs Γ A b B s₁ s₂ s₃ h₀ h₁ h₂ h₃, h₄, h₅ => by
-  apply typing.abs
-  apply h₀
-  apply weakening_typing h₁ h₄ h₅
-  apply weakening_typing h₂ (h₄.succ A) h₅
-  apply weakening_typing h₃ (h₄.succ A) h₅
-| .app Γ f A B a h₀ h₁, h₂, h₃ => by
+    . apply isItem_of_isInsert_of_le h₂ (by simpa using h) h₁.3
+| .sort _ s₁ s₂ h₀ h₁, h₂, h₃ =>
+    typing.sort _ _ _ h₀ (weakening_wf h₁ h₂ h₃)
+| .pi _ A B s₁ s₂ s₃ h₀ h₁ h₃, h₄, h₅ =>
+  typing.pi _ _ _ _ _ _ h₀ (weakening_typing h₁ h₄ h₅)
+    (weakening_typing h₃ (h₄.succ A) h₅)
+| .abs _ A b B s₁ s₂ s₃ h₀ h₁ h₂ h₃, h₄, h₅ =>
+  typing.abs _ _ _ _ _ _ _ h₀ (weakening_typing h₁ h₄ h₅)
+    (weakening_typing h₂ (h₄.succ A) h₅) (weakening_typing h₃ (h₄.succ A) h₅)
+| .app _ f B C b h₀ h₁, h₂, h₃ => by
   have : n = 0 + n := by simp
   rw [this, subst_lift]; simp
-  apply typing.app
-  apply weakening_typing h₀ h₂ h₃
-  apply weakening_typing h₁ h₂ h₃
-| .conv Γ a A B s h₀ h₁ h₂, h₃, h₄ => by
-  apply typing.conv _ _ (A ↑ 1 # n) _ _ h₀.lift
-  apply weakening_typing h₁ h₃ h₄
-  apply weakening_typing h₂ h₃ h₄
+  apply typing.app _ _ _ _ _ (weakening_typing h₀ h₂ h₃) (weakening_typing h₁ h₂ h₃)
+| .conv _ _ B _ s h₀ h₁ h₂, h₃, h₄ =>
+  typing.conv _ _ (B ↑ 1 # n) _ _ h₀.lift (weakening_typing h₁ h₃ h₄)
+    (weakening_typing h₂ h₃ h₄)
 
-def weakening_wf : ∀ (_ : Γ ⊢ ⬝) (_ : isInsert Δ A n Γ Γ') (_ : Δ ⊢ A : !s),
-    (Γ' ⊢ ⬝)
+def weakening_wf : Γ ⊢ ⬝ → isInsert Δ A n Γ Γ' → (Δ ⊢ A : !s) → (Γ' ⊢ ⬝ )
 | _, .zero, h₃ => wf.cons _ _ _ h₃
-| _, .succ u (Δ := Γ) (n := n) h₂, h₃ => by
+| .cons _ _ s _, .succ u (Δ := Γ) (n := n) h₂, h₃ => by
     rename_i h₁ _
-    cases h₁
-    rename_i s h₀
-    apply wf.cons _ _ s
-    have : (!s) = ((!s) ↑ 1 # n) := by rfl
-    rw [this]
-    apply weakening_typing h₀ h₂ h₃
+    apply wf.cons _ _ s (weakening_typing h₁ h₂ h₃)
 end
 
-#check ℕ
+def weakening_cons {Γ : PCtx S} {t T : PTerm S} {s : S.sort} (h₁ : Γ ⊢ t : T) (h₂ : Γ ⊢ A : !s) :
+    A :: Γ ⊢ t ↑ 1 : T ↑ 1 :=
+  weakening_typing h₁ isInsert.zero h₂
 
-def lift_inv_of_typing : ∀ (_ : Γ ⊢ t : T), (t ↑ 1 # Γ.length) = t
-| .var Γ T n h₁ ⟨B, h₂⟩ => by simp [h₂.2.lt_length]
+def weakening_isTrunc {Γ Γ' : PCtx S} {t T : PTerm S} :
+  ∀ (_ : isTrunc n Γ Γ') (_ : Γ' ⊢ t : T) (_ : Γ ⊢ ⬝), Γ ⊢ t ↑ n : T ↑ n
+| .zero _, _, _ => by simpa
+| .succ _ h₀, h₁, h₂ => by
+  rw [← lift0_lift0, ← lift0_lift0]
+  apply weakening_cons (weakening_isTrunc h₀ h₁ h₂.typing_of_cons.wf) h₂.typing_of_cons
+
+mutual
+
+def substitution_typing : ∀ (_ : Γ ⊢ t : T) (_ : isSubst Δ a A n Γ Γ') (_ : Δ ⊢ a : A),
+    Γ' ⊢ t{a//n} : T{a//n}
+| .var _ _ k h₀ h₁, h₂, h₃ => by
+  dsimp
+  split_ifs with h h'
+  . apply typing.var _ _ _ (substitution_wf h₀ h₂ h₃)
+    use h₁.1{a // n - (k + 1)}
+    . conv_lhs => rw [h₁.2]
+      rw [subst_lift_of_le _ _ _ (by simp)]
+      rw [← Nat.add_sub_assoc h, Nat.add_sub_cancel_left]
+    . apply isItem_of_isSubst_of_lt h₂ h h₁.3
+  . cases h'
+    have : T{a // n} = A ↑ n := by
+      obtain ⟨b, h₁, h₁'⟩ := h₁
+      rw [eq_of_isSubst_of_isItem h₂ h₁', h₁]
+      rw [lift_subst_of_le_of_le 0 _ _ (by simp) (by simp)]
+    rw [this]
+    apply weakening_isTrunc h₂.isTrunc h₃ (substitution_wf h₀ h₂ h₃)
+  . apply typing.var _ _ _ (substitution_wf h₀ h₂ h₃)
+    have : 1 ≤ k := by
+      apply Nat.add_one_le_of_lt
+      apply lt_of_le_of_lt (Nat.zero_le n) (lt_of_le_of_ne (le_of_not_lt h) (Ne.symm h'))
+    use h₁.1
+    . conv_lhs => rw [h₁.2]
+      rw [lift_subst_of_le_of_le 0 _ _ (by simp) (by simpa using h)]
+      rw [Nat.sub_add_cancel this]
+    . apply isItem_of_isSubst_of_le h₂ _
+        (by simpa [Nat.sub_add_cancel this] using h₁.3)
+      apply Nat.le_sub_one_of_lt (lt_of_le_of_ne (le_of_not_lt h) (Ne.symm h'))
+| .sort _ s₁ s₂ h₀ h₁, h₂, h₃ =>
+  typing.sort _ _ _ h₀ (substitution_wf h₁ h₂ h₃)
+| .pi _ A B s₁ s₂ s₃ h₀ h₁ h₃, h₄, h₅ =>
+  typing.pi _ _ _ _ _ _ h₀ (substitution_typing h₁ h₄ h₅)
+    (substitution_typing h₃ (h₄.succ A) h₅)
+| .abs _ A b B s₁ s₂ s₃ h₀ h₁ h₂ h₃, h₄, h₅ =>
+  typing.abs _ _ _ _ _ _ _ h₀ (substitution_typing h₁ h₄ h₅)
+    (substitution_typing h₂ (h₄.succ A) h₅) (substitution_typing h₃ (h₄.succ A) h₅)
+| .app _ f B C b h₀ h₁, h₂, h₃ => by
+  rw [subst0_subst]
+  apply typing.app _ _ _ _ _ (substitution_typing h₀ h₂ h₃) (substitution_typing h₁ h₂ h₃)
+| .conv _ _ B _ s h₀ h₁ h₂, h₃, h₄ =>
+  typing.conv _ _ (B{a//n}) _ _ h₀.substl (substitution_typing h₁ h₃ h₄)
+    (substitution_typing h₂ h₃ h₄)
+
+def substitution_wf : ∀ (_ : Γ ⊢ ⬝ ) (_ : isSubst Δ a A n Γ Γ') (_ : Δ ⊢ a : A), Γ' ⊢ ⬝
+| _, .zero, h₃ => h₃.wf
+| .cons _ _ s _, .succ (n := n) (Δ := Γ) (Δ' := Γ') u h₂, h₃ => by
+  rename_i h₁
+  apply wf.cons _ _ s (substitution_typing h₁ h₂ h₃)
+
+end
+
+def typing_of_isItem_of_isTrunc {Γ Γ' : PCtx S} {A : PTerm S} {n : ℕ} :
+  ∀ (_ : A ↓ n in Γ) (_ : isTrunc (n + 1) Γ Γ')  (_ : Γ ⊢ ⬝),
+    Σ s : S.sort, Γ' ⊢ A : !s
+| .zero _, .succ _ (.zero _), .cons _ _ s h => ⟨s, h⟩
+| .succ B h₀, .succ _ h₁, h₂ =>
+  typing_of_isItem_of_isTrunc h₀ h₁ h₂.typing_of_cons.wf
+
+lemma exists_typing_of_isItem_of_isTrunc {Γ Γ' : PCtx S} {A : PTerm S} {n : ℕ} :
+  ∀ (_ : A ↓ n in Γ) (_ : isTrunc (n + 1) Γ Γ')  (_ : Γ ⊢ ⬝),
+    ∃ s : S.sort, Nonempty (Γ' ⊢ A : !s)
+| h₁, h₂, h₃ => ⟨_, ⟨(typing_of_isItem_of_isTrunc h₁ h₂ h₃).2⟩⟩
+
+def typing_of_isItemLift {Γ : PCtx S} {A : PTerm S} {n : ℕ} :
+  ∀ (_ : A ↓ n sub Γ)  (_ : Γ ⊢ ⬝),
+    Σ s : S.sort, (Γ ⊢ A : !s) := by
+  intro ⟨B, h₁, h₂⟩ h₃
+  use (typing_of_isItem_of_isTrunc h₂ h₂.isTrunc.2 h₃).1
+  simpa [h₁] using weakening_isTrunc h₂.isTrunc.2
+    (typing_of_isItem_of_isTrunc h₂ h₂.isTrunc.2 h₃).2 h₃
+
+lemma exists_typing_of_isItemLift {Γ : PCtx S} {A : PTerm S} {n : ℕ} :
+  ∀ (_ : A ↓ n sub Γ)  (_ : Γ ⊢ ⬝),
+    ∃ s : S.sort, Nonempty (Γ ⊢ A : !s) := by
+  intro ⟨B, h₁, h₂⟩ h₃
+  obtain ⟨Γ', ⟨hΓ'⟩⟩ := exists_isTrunc_of_isItem h₂
+  obtain ⟨s, ⟨hs⟩⟩ := exists_typing_of_isItem_of_isTrunc h₂ hΓ' h₃
+  use s
+  constructor
+  simpa [h₁] using weakening_isTrunc hΓ' hs h₃
+
+lemma exists_eq_sort_or_typing_sort {Γ : PCtx S} {a A: PTerm S} : ∀ (_ : Γ ⊢ a : A),
+    (∃ s : S.sort, A = (!s)) ∨ (∃ s, Nonempty (Γ ⊢ A : !s))
+| .var Γ A i h₁ h₂ => by right; exact exists_typing_of_isItemLift h₂ h₁
+| .sort Γ s₁ s₂ h₁ h₂ => by left; exact ⟨_, rfl⟩
+| .conv _ _ _ _ _ _ _ h => by right; exact ⟨_, ⟨h⟩⟩
+| .app _ f A B a h₁ h₂ => by
+  rcases exists_eq_sort_or_typing_sort h₁ with ⟨s, h⟩ | ⟨s, ⟨h⟩⟩
+  . simp at h
+  . right
+    obtain ⟨s₁, s₂, s₃, ⟨h₃⟩, h₄, ⟨h₅⟩, ⟨h₆⟩⟩ := exists_of_pi_typing h
+    exact ⟨s₂, ⟨substitution_typing h₆ isSubst.zero h₂⟩⟩
+| .abs _ _ _ _ _ _ _  h₀ h₁ h₂ _ => by right; exact ⟨_, ⟨typing.pi _ _ _ _ _ _ h₀ h₁ h₂⟩⟩
+| .pi _ _ _ _ _ _ _ h₀ h₁ => by left; exact ⟨_, rfl⟩
+alias typing_correct := exists_eq_sort_or_typing_sort
+
+lemma exists_typing_sort_of_ne {Γ : PCtx S} {a A: PTerm S} (h₁ : Γ ⊢ a : A)
+    (h₂ : ∀ s : S.sort, A ≠ (!s)) : ∃ s, Nonempty (Γ ⊢ A : !s) := by
+  rcases exists_eq_sort_or_typing_sort h₁ with ⟨s, h⟩ | h
+  . simpa using h₂ s h
+  . exact h
+
+def typing_sort_of_ne {Γ : PCtx S} {a A: PTerm S} (h : ∀ s : S.sort, A ≠ !s) :
+    ∀ (_ : Γ ⊢ a : A), Σ s, Γ ⊢ A : !s
+| .var Γ A i h₁ h₂ => typing_of_isItemLift h₂ h₁
+| .sort Γ s₁ s₂ h₁ h₂ => by simp at h
+| .conv _ _ _ _ _ _ _ h' => ⟨_, h'⟩
+| .abs _ _ _ _ _ _ _  h₀ h₁ h₂ _ => ⟨_, typing.pi _ _ _ _ _ _ h₀ h₁ h₂⟩
+| .pi _ _ _ _ _ _ _ h₀ h₁ => by simp at h
+| .app _ f A B a h₁ h₂ =>
+  ⟨_ , substitution_typing (of_pi_typing (typing_sort_of_ne (by simp) h₁).2).typing₂
+    isSubst.zero h₂⟩
+
+def typing_sort_of_pi_typing {Γ : PCtx S} {a A B : PTerm S} :
+    ∀ (_ : Γ ⊢ a : Π.A B), Σ s : S.sort, Γ ⊢ Π.A B : !s
+| h => typing_sort_of_ne (by simp) h
+
+lemma lift_inv_of_typing : ∀ (_ : Γ ⊢ t : T), (t ↑ 1 # Γ.length) = t
+| .var Γ t n h₁ ⟨B, _, h₂⟩ => by simp [h₂.lt_length]
 | .sort _ _ _ _ _ => by simp
 | .conv _ _ _ _ _ _ h _ => lift_inv_of_typing h
 | .app _ _ _ _ _ h₁ h₂ => by
@@ -666,9 +1265,15 @@ def lift_inv_of_typing : ∀ (_ : Γ ⊢ t : T), (t ↑ 1 # Γ.length) = t
 | .pi _ _ _ _ _ _ _ h₀ h₁ => by
   simp; exact ⟨lift_inv_of_typing h₀, lift_inv_of_typing h₁⟩
 
-def lift_inv_of_typing'  (h : Γ ⊢ t : T) : (T ↑ 1 # Γ.length) = T := sorry
+lemma lift_inv_of_typing'  (h : Γ ⊢ t : T) :
+    (T ↑ 1 # Γ.length) = T := by
+  rcases typing_correct h with ⟨_, hs⟩ | ⟨_, ⟨hs⟩⟩
+  . simp [hs]
+  . apply lift_inv_of_typing hs
 
-def lift_inv_of_typing''  (h : T :: Γ ⊢ ⬝) : (T ↑ 1 # Γ.length) = T := sorry
+lemma lift_inv_of_typing''  (h : T :: Γ ⊢ ⬝) : (T ↑ 1 # Γ.length) = T := by
+  cases h
+  apply lift_inv_of_typing (by assumption)
 
 def isInsert_length : ∀ {Γ Δ : PCtx S} (_ : Δ ⊢ ⬝ ),
   isInsert Γ A (length Δ) (List.append Δ Γ) (List.append Δ (A :: Γ))
@@ -690,19 +1295,13 @@ def append_typing : ∀ {Γ Δ : PCtx S} (_ : Γ ⊢ ⬝) (_ : Δ ⊢ t : T),
 
 def append_wf : ∀ {Γ Δ : PCtx S} (_ : Γ ⊢ ⬝) (_ : Δ ⊢ ⬝), List.append Δ Γ ⊢ ⬝
 | _, [], h, _ => h
-| Γ, A :: Δ, h₁, .cons _ _ _ h₂ =>
+| _, _ :: _, h₁, .cons _ _ _ h₂ =>
   weakening_wf (append_wf h₁ (wf_of_typing h₂)) isInsert.zero
     (append_typing h₁ h₂)
 
 def weakening_cons_typing {Γ : PCtx S} {A : PTerm S} (h : A :: Γ ⊢ ⬝ ):
     Σs, (A :: Γ) ⊢ A ↑ 1 : !s :=
   ⟨_, weakening_typing (exists_of_cons' h).2 isInsert.zero (exists_of_cons' h).2⟩
-
-def substitution_typing : ∀ (_ : Γ ⊢ t : T) (_ : isSubst Δ a A n Γ Γ') (_ : Δ ⊢ a : A),
-  Γ' ⊢ t{a//n} : T{a//n} := sorry
-
-def substitution_wf : ∀ (_ : Γ ⊢ ⬝ ) (_ : isSubst Δ a A n Γ Γ') (_ : Δ ⊢ a : A),
-  Γ' ⊢ ⬝ := sorry
 
 end Typing
 
@@ -943,13 +1542,13 @@ inductive isSimulSubst : PCtx S → ℕ → PCtx S → PCtx S → Type _
 def simulSubst_wf (h : Γ' ⊢ ⬝) : ∀ (_ : isSimulSubst Γ' n F Γ),
     Γ ⊢ ⬝
 | .nil Γ n => h
-| .cons Γ n f F Γ' Γs Δ A s h₁ h₂ h₃ h₄ h₅ =>
+| .cons _ n f F Γ' _ Δ _ _ h₁ h₂ h₃ h₄ h₅ =>
   substitution_wf (simulSubst_wf h h₁) h₅ h₄
 
 def simulSubst_typing (h : Γ' ⊢ t : T) : ∀ (_ : isSimulSubst Γ' n F Γ),
     Γ ⊢ simulSubst t n F : simulSubst T n F
 | .nil Γ n => h
-| .cons Γ n f F Γ' Γs Δ A s h₁ h₂ h₃ h₄ h₅ =>
+| .cons _ n f F Γ' _ Δ _ _ h₁ h₂ h₃ h₄ h₅ =>
   substitution_typing (simulSubst_typing h h₁) h₅ h₄
 
 inductive isMor (Γ : PCtx S) : PCtx S → PCtx S → Type _
@@ -995,7 +1594,7 @@ lemma isSubst.length_lt {Γ Δ Δ' : PCtx S} (h : isSubst Γ f A n Δ Δ') :
 lemma isSimulSubst.length_le {Γ F Δ : PCtx S} : ∀ (_ : isSimulSubst Γ n F Δ),
     Δ.length ≤ Γ.length
 | .nil Γ n => le_refl _
-| .cons Γ n f F Γ' Γs Δ A s h₁ h₂ h₃ h₄ h₅ =>
+| .cons _ n f F Γ' _ Δ _ _ h₁ h₂ h₃ h₄ h₅ =>
   h₅.length_lt.le.trans h₁.length_le
 
 lemma isSimulSubst.nil_of_nil {F Δ : PCtx S} (h : isSimulSubst [] n F Δ) :
@@ -1148,7 +1747,7 @@ lemma nil_pcomp : ∀ {G : PCtx S}, pcomp [] G = G
 | [] => rfl
 | g :: G => by simp [pcomp]; rw [nil_pcomp]
 
-lemma simulSubst_pcomp {Γ Δ Θ : PCtx S} {T : PTerm S} (h : Θ' ⊢ T : !s):
+lemma simulSubst_pcomp {Γ Δ Θ Θ': PCtx S} {T : PTerm S} (h : (T ↑ 1 # length Θ') = T):
   ∀ {F G : PCtx S} (_ : isMor Γ Δ F) (_ : isMor Δ Θ G) (_ : isTrunc k Θ' Θ),
   simulSubst T k (pcomp F G) = simulSubst (simulSubst T k G) k F
 | F, [], h₁, h₂, h₃ => by
@@ -1156,7 +1755,7 @@ lemma simulSubst_pcomp {Γ Δ Θ : PCtx S} {T : PTerm S} (h : Θ' ⊢ T : !s):
   cases h₂
   rw [liftinv (le_refl _)]
   rw [← h₃.nil_length]
-  apply lift_inv_of_typing h
+  apply h
 | [], G, h₁, h₂, h₃ => by
   cases h₁
   simp
@@ -1187,7 +1786,7 @@ def pcomp_isMor {Γ : PCtx S} : ∀ {Δ Θ F G : PCtx S} (_ : Γ ⊢ ⬝) (_ : �
   simpa [simulSubst_sort] using simulSubst_typing (append_typing hΓ h₃) (isMor'_isMor h₁)
   apply simulSubst_typing (append_typing hΓ h₄) (isMor'_isMor h₁)
   convert isSubst.zero using 2
-  apply simulSubst_pcomp (exists_of_cons' hΘ).snd h₁ h₂ (isTrunc.zero _)
+  apply simulSubst_pcomp (lift_inv_of_typing'' hΘ) h₁ h₂ (isTrunc.zero _)
 
 end pcomp
 
@@ -1195,7 +1794,7 @@ section id
 
 
 @[simp]
-def idN : ℕ → ℕ →  PCtx S
+def idN : ℕ → ℕ → PCtx S
 | _, 0 => []
 | n, k + 1 => (#n) :: (idN (n + 1) k)
 
@@ -1361,14 +1960,18 @@ lemma isMorAuxLift {k l m} : ∀ {A : PTerm S} (_ : (A ↑ 1 # m) = A),
     simp [simulSubst_app] at h ⊢
     exact ⟨isMorAuxLift h.1, isMorAuxLift h.2⟩
 
-def aux₁wf (h : A :: Γ ⊢ ⬝) : (A ↑ 1 # Γ.length) = A := by
-  cases h
-  apply lift_inv_of_typing (by assumption)
+def simulSubst_id_of_cons_wf :
+    (_ : A :: Γ ⊢ ⬝) → simulSubst A 0 (id Γ) = A
+| .cons _ _ _ h => by
+  simp [id, id₀]
+  rw [isMorAuxLift, lift_zero]
+  apply lift_inv_of_typing h
 
-def simulSubst_id_cons (h : A :: Γ ⊢ ⬝) :
-    simulSubst A 0 (id Γ) = A := by
-  conv_rhs => rw [← lift_zero (M := A) (c := 0)]
-  apply isMorAuxLift (aux₁wf h)
+def simulSubst_id_of_typing {Γ : PCtx S} {f A : PTerm S} (h : Γ ⊢ f : A) :
+    simulSubst f 0 (id Γ) = f := by
+  simp [id, id₀]
+  rw [isMorAuxLift, lift_zero]
+  apply lift_inv_of_typing h
 
 def wf_of_isTrunc {k} {Γ Δ : PCtx S} : ∀ (_ : isTrunc k Γ Δ) (_ : Γ ⊢ ⬝),
     Δ ⊢ ⬝
@@ -1379,11 +1982,9 @@ def wf_of_isTrunc {k} {Γ Δ : PCtx S} : ∀ (_ : isTrunc k Γ Δ) (_ : Γ ⊢ �
   apply wf_of_typing (by assumption)
 
 def isMorAux {k} {Γ Δ : PCtx S} {A} (h₀ : isTrunc k Γ (A :: Δ)) (h₁ : Γ ⊢ ⬝) :
-    Γ ⊢ #k : simulSubst A 0 (id₀ (k + 1) Δ) := by
-  refine typing.var _ _ _ h₁ ⟨A, ⟨?_, isIerm_of_isTrunc h₀⟩⟩
-  apply isMorAuxLift
-  apply aux₁wf
-  apply wf_of_isTrunc h₀ h₁
+    Γ ⊢ #k : simulSubst A 0 (id₀ (k + 1) Δ) :=
+  typing.var _ _ _ h₁ ⟨A,
+    isMorAuxLift (lift_inv_of_typing (wf_of_isTrunc h₀ h₁).typing_of_cons), isTrunc.isItem h₀⟩
 
 def id₀_isMor : ∀ {Γ Δ : PCtx S} (_ : isTrunc k Γ Δ) (_ : Γ ⊢ ⬝), isMor Γ Δ (id₀ k Δ)
 | Γ, [], h, h' => by apply isMor.nil
@@ -1407,10 +2008,6 @@ end id
 
 section
 -- weakening of isMor
-
-#check weakening_wf
-
-#check subst_lift
 
 lemma simulSubst_lift {A : PTerm S} {k : ℕ}  :
   ∀ {F : PCtx S} (_ : (A ↑ 1 # k + F.length) = A),
@@ -1504,11 +2101,21 @@ lemma zero_cons_pcomp_zero_cons {F G : PCtx S} (h : (G ↑↑ 1 # F.length) = G)
   . rw [simulSubst_var_of_lt (by simp)]; rfl
   . apply zero_cons_pcomp_zero_cons_aux₂ h
 
+lemma cons_pcomp_lift_one {F : PCtx S} : ∀ {G : PCtx S},
+    pcomp (A :: F) (G ↑↑ 1) = pcomp F G
+| [] => by rfl
+| g :: G => by
+  simp [pcomp]
+  congr 1
+  . rw [zero_cons_pcomp_zero_cons_aux₁, lift_subst_of_le_of_le 0 _ _ (by simp) (by simp),
+      lift_zero]
+  . apply cons_pcomp_lift_one
+
 end
 
 section
 
-def pcomp_id₀_aux : ∀ {F G : PCtx S} (_ : isTrunc k F G), pcomp F (id₀ k G) = G
+lemma pcomp_id₀_aux : ∀ {F G : PCtx S} (_ : isTrunc k F G), pcomp F (id₀ k G) = G
 | F, [], h => rfl
 | F, g :: G, h => by
   simp [pcomp]
@@ -1516,52 +2123,259 @@ def pcomp_id₀_aux : ∀ {F G : PCtx S} (_ : isTrunc k F G), pcomp F (id₀ k G
   apply simulSubst_var_of_isTrunc h
   apply pcomp_id₀_aux h.pred
 
-def pcomp_id₀ {F G Δ : PCtx S} (h : isTrunc k F G) (h' : Δ.length = G.length) :
+lemma pcomp_id₀ {F G Δ : PCtx S} (h : isTrunc k F G) (h' : Δ.length = G.length) :
     pcomp F (id₀ k Δ) = G := by
   convert pcomp_id₀_aux h using 2
   simp [id₀, id, h']
 
-def pcomp_id {Γ Δ F : PCtx S} (h : isMor Γ Δ F) : pcomp F (id Δ) = F := by
-  apply pcomp_id₀ (isTrunc.zero _) h.length_eq
+lemma pcomp_id {Γ Δ F : PCtx S} (h : isMor Γ Δ F) : pcomp F (id Δ) = F :=
+  pcomp_id₀ (isTrunc.zero _) h.length_eq
+
+lemma idN_pcomp {k n : ℕ} : ∀ {F : PCtx S} (_ : (F ↑↑ 1 # n) = F),
+    pcomp (idN k n) F = F ↑↑ k
+| [], _ => rfl
+| A :: F, h => by
+  simp only [pcomp]
+  apply List.cons.inj at h
+  rw [idN_pcomp h.2, isMorAuxLift h.1]
+  rfl
+
+lemma id₀_pcomp {k : ℕ} : ∀ {F G : PCtx S} (_ : (F ↑↑ 1 # G.length) = F),
+    pcomp (id₀ k G) F = F ↑↑ k :=
+  idN_pcomp
+
+lemma id_pcomp : ∀ {Γ Δ F : PCtx S} (_ : isMor Γ Δ F), pcomp (id Γ) F = F
+| Γ, _, _, .nil => rfl
+| Γ, D :: Δ, f :: F, .cons h₁ h₂ h₃ => by
+  simp only [pcomp, id_pcomp h₁, simulSubst_id_of_typing h₃]
+
+lemma pcomp_pcomp {Γ Δ Θ Κ: PCtx S}: ∀ {F G H : PCtx S}
+  (_ : isMor Γ Δ F) (_ : isMor Δ Θ G) (_ : isMor Θ Κ H)
+  , pcomp (pcomp F G) H = pcomp F (pcomp G H)
+| F, G, [], _, _, _ => by simp [pcomp]
+| F, G, h :: H, h₁, h₂, .cons h₃ h₄ h₅ => by
+  simp only [pcomp, simulSubst_pcomp (lift_inv_of_typing h₅) h₁ h₂ (isTrunc.zero _),
+    pcomp_pcomp h₁ h₂ h₃]
 
 end
 
-section
+noncomputable section
 
--- typing correct
-lemma typing_correct {Γ : PCtx S} {a A: PTerm S} : ∀ (_ : Γ ⊢ a : A),
-    (∃ s : S.sort, A = (!s)) ∨ (∃ s, Nonempty (Γ ⊢ A : !s)) := sorry
+namespace PCtx.beta
 
-def ctx_beta_typing {Γ Γ' : PCtx S} (h₁ : Γ ⊢ a : A) (h₂ : Γ' ⊢ ⬝) (h₃ : Γ →β Γ') :
-    Γ' ⊢ a : A := sorry
+@[simp]
+def nat {Γ Δ : PCtx S} : (Γ →β Δ) → ℕ
+| .head _ => 0
+| .tail h => h.nat + 1
 
-def ctx_beta_exp_typing {Γ Γ' : PCtx S} (h₁ : Γ ⊢ a : A) (h₂ : Γ' ⊢ ⬝) (h₃ : Γ' →β Γ) :
-    Γ' ⊢ a : A := sorry
+def pterml {Γ Δ : PCtx S} : (Γ →β Δ) → PTerm S
+| .head (A := A) _ => A
+| .tail h => h.pterml
 
-def term_betar_typing : ∀ {Γ : PCtx S} {t s M} (_: Γ ⊢ t : M) (_ : t ↠β s), Γ ⊢ s : M := sorry
+def ptermr {Γ Δ : PCtx S} : (Γ →β Δ) → PTerm S
+| .head (B := B) _ => B
+| .tail h => h.ptermr
+
+def pctx {Γ Δ : PCtx S} : (Γ →β Δ) → PCtx S
+| .head (Γ := Γ) _ => Γ
+| .tail h => h.pctx
+
+def ptermBeta {Γ Δ : PCtx S} : (h : Γ →β Δ) → (h.pterml →β h.ptermr)
+| .head h' => h'
+| .tail h => h.ptermBeta
+
+def isIteml {Γ Δ : PCtx S} : (h : Γ →β Δ) → h.pterml ↓ h.nat in Γ
+| .head _ => isItem.zero _
+| .tail h => isItem.succ _ h.isIteml
+
+def isTruncl {Γ Δ : PCtx S} : (h : Γ →β Δ) → isTrunc (h.nat + 1) Γ h.pctx
+| .head _ => isTrunc.succ _ (isTrunc.zero _)
+| .tail h => isTrunc.succ _ h.isTruncl
+
+def isItemr {Γ Δ : PCtx S} : (h : Γ →β Δ) → h.ptermr ↓ h.nat in Δ
+| .head _ => isItem.zero _
+| .tail h => isItem.succ _ h.isItemr
+
+def isTruncr {Γ Δ : PCtx S} : (h : Γ →β Δ) → isTrunc (h.nat + 1) Δ h.pctx
+| .head _ => isTrunc.succ _ (isTrunc.zero _)
+| .tail h => isTrunc.succ _ h.isTruncr
+
+def isItem_of_ne {Γ Δ : PCtx S} {A : PTerm S} :
+    {n : ℕ} → (h : Γ →β Δ) → (n ≠ h.nat) → (A ↓ n in Γ) → (A ↓ n in Δ)
+| 0, .head _, h₂, h₃ => by simp at h₂
+| n + 1, .head _, h₂, h₃ => isItem.succ _ h₃.pred
+| 0, .tail _, h₂, .zero _ => isItem.zero _
+| n + 1, .tail h₁, h₂, h₃ => by
+  apply isItem.succ
+  apply isItem_of_ne h₁ _ h₃.pred
+  simpa using h₂
+
+def isItemLift_of_ne {Γ Δ : PCtx S} {A : PTerm S} {n : ℕ} :
+    (h : Γ →β Δ) → (n ≠ h.nat) → (A ↓ n sub Γ) → (A ↓ n sub Δ)
+| h₁, h₂, ⟨B, h₃, h₄⟩ => by
+  exact ⟨_, h₃, h₁.isItem_of_ne h₂ h₄⟩
+
+def exp_isItem_of_ne {Γ Δ : PCtx S} {A : PTerm S} :
+    {n : ℕ} → (h : Γ →β Δ) → (n ≠ h.nat) → (A ↓ n in Δ) → (A ↓ n in Γ)
+| 0, .head _, h₂, h₃ => by simp at h₂
+| n + 1, .head _, h₂, h₃ => isItem.succ _ h₃.pred
+| 0, .tail _, h₂, .zero _ => isItem.zero _
+| n + 1, .tail h₁, h₂, h₃ => by
+  apply isItem.succ
+  apply exp_isItem_of_ne h₁ _ h₃.pred
+  simpa using h₂
+
+def exp_isItemLift_of_ne {Γ Δ : PCtx S} {A : PTerm S} {n : ℕ} :
+    (h : Γ →β Δ) → (n ≠ h.nat) → (A ↓ n sub Δ) → (A ↓ n sub Γ)
+| h₁, h₂, ⟨B, h₃, h₄⟩ => by
+  exact ⟨_, h₃, h₁.exp_isItem_of_ne h₂ h₄⟩
+
+end PCtx.beta
+
+def ctx_beta_typing_var_eq {Γ Γ' : PCtx S} {A : PTerm S} :
+  {n : ℕ} → (Γ ⊢ ⬝) → (Γ' ⊢ ⬝) → (h₃ : Γ →β Γ') → (A ↓ n sub Γ) → (n = h₃.nat)
+  → (Γ' ⊢ #n : A)
+| n, h₁, h₂, h₃, ⟨B, h₄, h₅⟩, h₆ => by
+  cases h₆
+  cases isItem_unique h₅ h₃.isIteml
+  cases h₄
+  apply typing.conv _ _ _ _ _ (h₃.ptermBeta.betac.symm).lift
+  apply typing.var _ _ _ h₂ ⟨_, rfl, h₃.isItemr⟩
+  exact weakening_isTrunc h₃.isTruncr (typing_of_isItem_of_isTrunc h₅ h₃.isTruncl h₁).2 h₂
+
+def ctx_beta_typing_var_ne {Γ Γ' : PCtx S} {A : PTerm S} :
+  {n : ℕ} → (Γ' ⊢ ⬝) → (h₃ : Γ →β Γ') → (A ↓ n sub Γ) → (n ≠ h₃.nat)
+  → (Γ' ⊢ #n : A)
+| _, h₁, h₂, h₃, h₄ => typing.var _ _ _ h₁ (h₂.isItemLift_of_ne h₄ h₃)
+
+def ctx_beta_typing_var {Γ Γ' : PCtx S} {A : PTerm S} :
+  {n : ℕ} → (Γ ⊢ ⬝) → (Γ' ⊢ ⬝) → (Γ →β Γ') → (A ↓ n sub Γ) → (Γ' ⊢ #n : A)
+| n, h₁, h₂, h₃, h₄ =>
+  if h : n = h₃.nat then ctx_beta_typing_var_eq h₁ h₂ h₃ h₄ h
+    else ctx_beta_typing_var_ne h₂ h₃ h₄ h
+
+def ctx_beta_typing {Γ Γ' : PCtx S} {a A : PTerm S} :
+    ∀ (_ : Γ ⊢ a : A) (_ : Γ' ⊢ ⬝) (_ : Γ →β Γ'), Γ' ⊢ a : A
+| .var _ _ _ h₁ h₂, h₃, h₄ => ctx_beta_typing_var h₁ h₃ h₄ h₂
+| .sort _ _ _ h₁ _, h₃, _ => typing.sort _ _ _ h₁ h₃
+| .pi _ _ _ _ _ _ h₁ h₂ h₃, h₄, h₅ => by
+  apply typing.pi _ _ _ _ _ _ h₁
+  apply ctx_beta_typing h₂ h₄ h₅
+  apply ctx_beta_typing h₃ (wf.cons _ _ _ (ctx_beta_typing h₂ h₄ h₅)) (PCtx.beta.tail h₅)
+| .abs _ _ _ _ _ _ _ h₀ h₁ h₂ h₃, h₄, h₅ => by
+  apply typing.abs _ _ _ _ _ _ _ h₀
+  apply ctx_beta_typing h₁ h₄ h₅
+  apply ctx_beta_typing h₂ (wf.cons _ _ _ (ctx_beta_typing h₁ h₄ h₅)) (PCtx.beta.tail h₅)
+  apply ctx_beta_typing h₃ (wf.cons _ _ _ (ctx_beta_typing h₁ h₄ h₅)) (PCtx.beta.tail h₅)
+| .app _ _ _ _ _ h₁ h₂, h₃, h₄ =>
+  typing.app _ _ _ _ _ (ctx_beta_typing h₁ h₃ h₄) (ctx_beta_typing h₂ h₃ h₄)
+| .conv _ _ _ _ _ h₁ h₂ h₃, h₄, h₅ =>
+  typing.conv _ _ _ _ _ h₁ (ctx_beta_typing h₂ h₄ h₅) (ctx_beta_typing h₃ h₄ h₅)
+
+def ctx_beta_exp_typing_var_eq {Γ Γ' : PCtx S} {A : PTerm S} :
+  {n : ℕ} → (Γ ⊢ ⬝) → (Γ' ⊢ ⬝) → (h₃ : Γ' →β Γ) → (A ↓ n sub Γ) → (n = h₃.nat)
+  → (Γ' ⊢ #n : A)
+| n, h₁, h₂, h₃, ⟨B, h₄, h₅⟩, h₆ => by
+  cases h₆
+  cases isItem_unique h₅ h₃.isItemr
+  cases h₄
+  apply typing.conv _ _ _ _ _ (h₃.ptermBeta.betac).lift
+  apply typing.var _ _ _ h₂ ⟨_, rfl, h₃.isIteml⟩
+  exact weakening_isTrunc h₃.isTruncl (typing_of_isItem_of_isTrunc h₅ h₃.isTruncr h₁).2 h₂
+
+def ctx_beta_exp_typing_var_ne {Γ Γ' : PCtx S} {A : PTerm S} :
+  {n : ℕ} → (Γ' ⊢ ⬝) → (h₃ : Γ' →β Γ) → (A ↓ n sub Γ) → (n ≠ h₃.nat)
+  → (Γ' ⊢ #n : A)
+| _, h₁, h₂, h₃, h₄ => typing.var _ _ _ h₁ (h₂.exp_isItemLift_of_ne h₄ h₃)
+
+def ctx_beta_exp_typing_var {Γ Γ' : PCtx S} {A : PTerm S} :
+  {n : ℕ} → (Γ ⊢ ⬝) → (Γ' ⊢ ⬝) → (Γ' →β Γ) → (A ↓ n sub Γ) → (Γ' ⊢ #n : A)
+| n, h₁, h₂, h₃, h₄ =>
+  if h : n = h₃.nat then ctx_beta_exp_typing_var_eq h₁ h₂ h₃ h₄ h
+    else ctx_beta_exp_typing_var_ne h₂ h₃ h₄ h
+
+def ctx_beta_exp_typing {Γ Γ' : PCtx S} {a A : PTerm S} :
+    ∀ (_ : Γ ⊢ a : A) (_ : Γ' ⊢ ⬝) (_ : Γ' →β Γ), Γ' ⊢ a : A
+| .var _ _ _ h₁ h₂, h₃, h₄ => ctx_beta_exp_typing_var h₁ h₃ h₄ h₂
+| .sort _ _ _ h₁ _, h₃, _ => typing.sort _ _ _ h₁ h₃
+| .pi _ _ _ _ _ _ h₁ h₂ h₃, h₄, h₅ => by
+  apply typing.pi _ _ _ _ _ _ h₁
+  apply ctx_beta_exp_typing h₂ h₄ h₅
+  apply ctx_beta_exp_typing h₃ (wf.cons _ _ _ (ctx_beta_exp_typing h₂ h₄ h₅)) (PCtx.beta.tail h₅)
+| .abs _ _ _ _ _ _ _ h₀ h₁ h₂ h₃, h₄, h₅ => by
+  apply typing.abs _ _ _ _ _ _ _ h₀
+  apply ctx_beta_exp_typing h₁ h₄ h₅
+  apply ctx_beta_exp_typing h₂ (wf.cons _ _ _ (ctx_beta_exp_typing h₁ h₄ h₅)) (PCtx.beta.tail h₅)
+  apply ctx_beta_exp_typing h₃ (wf.cons _ _ _ (ctx_beta_exp_typing h₁ h₄ h₅)) (PCtx.beta.tail h₅)
+| .app _ _ _ _ _ h₁ h₂, h₃, h₄ =>
+  typing.app _ _ _ _ _ (ctx_beta_exp_typing h₁ h₃ h₄) (ctx_beta_exp_typing h₂ h₃ h₄)
+| .conv _ _ _ _ _ h₁ h₂ h₃, h₄, h₅ =>
+  typing.conv _ _ _ _ _ h₁ (ctx_beta_exp_typing h₂ h₄ h₅) (ctx_beta_exp_typing h₃ h₄ h₅)
+
+def term_beta_typing {Γ : PCtx S} {t s M : PTerm S} :
+    ∀ (_: Γ ⊢ t : M) (_ : t →β s), Γ ⊢ s : M
+| .pi _ _ _ _ _ _ h₁ h₂ h₃, .pil _ _ _ h₄ =>
+  typing.pi _ _ _ _ _ _ h₁ (term_beta_typing h₂ h₄)
+    (ctx_beta_typing h₃ (wf.cons _ _ _ (term_beta_typing h₂ h₄)) (PCtx.beta.head h₄))
+| .pi _ _ _ _ _ _ h₁ h₂ h₃, .pir _ _ _ h₄ =>
+  typing.pi _ _ _ _ _ _ h₁ h₂ (term_beta_typing h₃ h₄)
+| .abs _ _ _ B _ _ _ h₀ h₁ h₂ h₃, .absl _ A' _ h₄ => by
+  apply typing.conv _ _ _ _ _ (beta.pil _ _ B h₄).betac.symm
+  apply typing.abs _ _ _ _ _ _ _ h₀ (term_beta_typing h₁ h₄)
+    (ctx_beta_typing h₂ (wf.cons _ _ _ (term_beta_typing h₁ h₄)) (PCtx.beta.head h₄))
+    (ctx_beta_typing h₃ (wf.cons _ _ _ (term_beta_typing h₁ h₄)) (PCtx.beta.head h₄))
+  apply (typing.pi _ _ _ _ _ _ h₀ h₁ h₂)
+| .abs _ _ _ _ _ _ _ h₀ h₁ h₂ h₃, .absr _ _ _ h₄ =>
+  typing.abs _ _ _ _ _ _ _ h₀ h₁ h₂ (term_beta_typing h₃ h₄)
+| .app _ _ _ _ _ h₁ h₂, .red _ _ _ => by
+  apply typing.conv _ _ _ _ _ ((pi_inj (of_abs_typing h₁).betac).2.symm).substl
+  apply substitution_typing (of_abs_typing h₁).typing₃ isSubst.zero
+  apply typing.conv _ _ _ _ _ (pi_inj (of_abs_typing h₁).betac).1 h₂
+    (of_abs_typing h₁).typing₁
+  apply substitution_typing (of_pi_typing (typing_sort_of_pi_typing h₁).2).typing₂ isSubst.zero h₂
+| .app _ _ _ _ _ h₁ h₂, .appl _ _ _ h₄ =>
+  typing.app _ _ _ _ _ (term_beta_typing h₁ h₄) h₂
+| .app _ _ _ _ _ h₁ h₂, .appr _ _ _ h₄ => by
+  apply typing.conv _ _ _ _ _ (h₄.betac.symm).substr
+  apply typing.app _ _ _ _ _ h₁ (term_beta_typing h₂ h₄)
+  apply substitution_typing (of_pi_typing (typing_sort_of_pi_typing h₁).2).typing₂ isSubst.zero h₂
+| .conv _ _ _ _ _ h₁ h₂ h₃, h₄ =>
+  typing.conv _ _ _ _ _ h₁ (term_beta_typing h₂ h₄) h₃
+
+def term_betar_typing {Γ : PCtx S} {t s M : PTerm S} :
+    ∀ (_: Γ ⊢ t : M) (_ : t ↠β s), Γ ⊢ s : M
+| h₁, .beta _ _ h₂ => term_beta_typing h₁ h₂
+| h₁, .refl _ => h₁
+| h₁, .trans _ _ _ h₂ h₃ => term_betar_typing (term_betar_typing h₁ h₂) h₃
 alias subject_reduction := term_betar_typing
 
-def betac_of_pi_betac : ∀ {A B A' B' : PTerm S} (_ : Π.A B ≃β Π.A' B'),
-    A ≃β A' × B ≃β B' := sorry
-alias pi_inj := betac_of_pi_betac
+def ctx_beta_wf :
+  ∀ {Γ Γ' : PCtx S} (_ : Γ ⊢ ⬝) (_ : Γ →β Γ'), Γ' ⊢ ⬝
+| [], [], _, _ => wf.nil
+| [], _ :: _, _, h => by simpa using h.length_eq
+| _ :: _, [], _, h => by simpa using h.length_eq
+| _ :: _, _ :: _, .cons _ _ _ h, .head h' => wf.cons _ _ _ (term_beta_typing h h')
+| _ :: _, _ :: _, .cons _ _ _ h, .tail h' =>
+  wf.cons _ _ _ (ctx_beta_typing h (ctx_beta_wf h.wf h') h')
 
-def ctx_beta_wf {Γ Γ' : PCtx S} (h₁ : Γ ⊢ ⬝) (h₂ : Γ' →β Γ) :
-    Γ' ⊢ ⬝ := sorry
+def ctx_betar_wf {Γ Γ' : PCtx S} :
+    ∀ (_ : Γ ⊢ ⬝) (_ : Γ ↠β Γ'), Γ' ⊢ ⬝
+| h, .beta _ _ h' => ctx_beta_wf h h'
+| h, .refl _ => h
+| h, .trans _ _ _ h₁ h₂ => ctx_betar_wf (ctx_betar_wf h h₁) h₂
 
-def ctx_betar_wf {Γ Γ' : PCtx S} (h₁ : Γ ⊢ ⬝) (h₂ : Γ' ↠β Γ) :
-    Γ' ⊢ ⬝ := sorry
-
-def ctx_betar_typing {Γ Γ' : PCtx S} (h₁ : Γ ⊢ a : A) : ∀ (h₃ : Γ ↠β Γ'),
+def ctx_betar_typing {Γ Γ' : PCtx S} : ∀ (_ : Γ ⊢ a : A) (_ : Γ ↠β Γ'),
     Γ' ⊢ a : A
-| .beta _ _ h => sorry
-| .refl _ => h₁
-| .trans _ _ _ h₃ h₄ => sorry
+| h, .beta _ _ h' => ctx_beta_typing h (ctx_betar_wf h.wf (PCtx.betar.beta _ _ h')) h'
+| h, .refl _ => h
+| h, .trans _ _ _ h₁ h₂ => ctx_betar_typing (ctx_betar_typing h h₁) h₂
 
-def ctx_betar_exp_typing {Γ Γ' : PCtx S} (h₁ : Γ ⊢ a : A) (h₂ : Γ' ⊢ ⬝) : ∀ (h₃ : Γ' ↠β Γ),
+def ctx_betar_exp_typing {Γ Γ' : PCtx S} : ∀ (_ : Γ ⊢ a : A) (_ : Γ' ⊢ ⬝) (_ : Γ' ↠β Γ),
     Γ' ⊢ a : A
-| .beta _ _ h => sorry
-| .refl _ => h₁
-| .trans _ _ _ h₃ h₄ => sorry
+| h₁, h₂, .beta _ _ h₃ => ctx_beta_exp_typing h₁ h₂ h₃
+| h₁, h₂, .refl _ => h₁
+| h₁, h₂, .trans _ _ _ h₃ h₄ =>
+  ctx_betar_exp_typing (ctx_betar_exp_typing h₁ (ctx_betar_wf h₂ h₃) h₄) h₂ h₃
 
 def ctx_betac_confl : ∀ {Γ Δ : PCtx S} (_ : Γ ≃β Δ),
     Σ (Θ : PCtx S), (Γ ↠β Θ) × (Δ ↠β Θ)
@@ -1590,7 +2404,7 @@ section
 -- `isMor` is sound wrt to `betac`
 
 def isMor_betac₁ {Γ Γ' : PCtx S} (h₁ : Γ' ⊢ ⬝) (h₂ : Γ ≃β Γ'):
-  ∀ {Δ F : PCtx S} (h₃ : isMor Γ Δ F), isMor Γ' Δ F
+  ∀ {Δ F : PCtx S} (_ : isMor Γ Δ F), isMor Γ' Δ F
 | [], _, h => by cases h.of_nil; apply isMor.nil
 | _, [], h => by cases h.of_mor_nil; apply isMor.nil
 | D :: Δ, f :: F, .cons h₃ h₄ h₅ =>
