README.md
@@ -1,44 +1,44 @@
 # HoTT_Model
 
-This repository aims to formalize [the simplcial model of HoTT](https://arxiv.org/abs/1211.2851). All the indexes below refer to this paper.
+This repository aims to formalize [the simplicial model of HoTT](https://arxiv.org/abs/1211.2851). All the indexes below refer to this paper.
 
 ## On the semantic side:
 
 ### Contextual Category
-- [x] Contextual catgory (1.2.1)
-- [x] Logical sturctures on a contextual catgory (Appendix B)
+- [x] Contextual category (1.2.1)
+- [x] Logical structures on a contextual category (Appendix B)
 
 ### Universe
 - [x] Universe in a category, i.e., a morphism with chosen pullbacks (1.3)
 - [x] Universe induces a contextual category (1.3.2, 1.3.3)
-- Logical sturctures on a universe in a locally closed cartesian category (1.4)
+- Logical structures on a universe in a locally closed cartesian category (1.4)
 - If the universe has a certain logical structures, so does the contextual category it induces (1.4.15)
 - [x] $\Pi$-type has been completely formalized for the last two points.
 
-### The simplcial model
+### The simplicial model
 1. Construction
 - [x] $\alpha$-small well-ordered morphisms of simplicial sets (2.1.1, 2.1.3)
 - [x] The isomorphism classes form a set, or is `Small` in Lean. (Footnote 9)
 - [x] The isomorphism classes form a functor $\mathbf W_{\alpha}$ from simplicial sets to sets, and the functor preserves limits (2.1.4)
 - [x] The functor is represented by $W_\alpha$ (2.1.5)
 - [x] The canonical map $\tilde W_\alpha \to W_\alpha$ is strictly universal with respect to all the $\alpha$-small well-ordered morphisms
-- [x] The subobject $U_\alpha$ correpsonding to all the $\alpha$-small well-ordered Kan fibrations and a map $\tilde U_\alpha \to U_\alpha$ (2.1.9)
+- [x] The subobject $U_\alpha$ corresponding to all the $\alpha$-small well-ordered Kan fibrations and a map $\tilde U_\alpha \to U_\alpha$ (2.1.9)
 - [x] $\tilde U_\alpha \to U_\alpha$ is a Kan fibration (2.1.10)
 - [x] $\tilde U_\alpha \to U_\alpha$ is strictly universal with respect to all the $\alpha$-small well-ordered Kan fibrations (2.1.12)
 - [x] $\tilde U_\alpha \to U_\alpha$ forms a universe
 - [x] Dependent products of a small morphism along a small morphism is again small.
 
 2. Property
-- The universe given by $\tilde U_\alpha \to U_\alpha$ has the logical sturctures
+- The universe given by $\tilde U_\alpha \to U_\alpha$ has the logical structures
 - The contextual category satisfies univalence
 
 ### Locally cartesian closedness
-- [x] Defintion of locally cartesian closed categories ([Referenece](https://github.com/sinhp/Poly))
-- [x] Every presheaf catgeory is locally cartesian closed categories. Here by presheaf catgeory we mean`Cᵒᵖ ⥤ Type max v w`, where the type of morphisms of `C` lies in `Type v`, hence not neccessarily `Cᵒᵖ ⥤ Type v`. In particular `SSet.{u}` is locally cartesian closed for any `u`.
+- [x] Definition of locally cartesian closed categories ([Reference](https://github.com/sinhp/Poly))
+- [x] Every presheaf category is locally cartesian closed categories. Here by presheaf category we mean`Cᵒᵖ ⥤ Type max v w`, where the type of morphisms of `C` lies in `Type v`, hence not necessarily `Cᵒᵖ ⥤ Type v`. In particular `SSet.{u}` is locally cartesian closed for any `u`.
 - [x] A not so trivial lemma: dependent products of a pullback along a pullback is a pullback.
 
 ## On the syntactic side
 - Aim to formalize a type theory. Since formalizing the whole Martin-Löf type theory would be too much work, only
 	trying [pure type system](https://ncatlab.org/nlab/show/pure+type+system) now
-- Aim to define a contextual category of well-fromed contexts of PTS. (Almost done)
-- Aim to define an interpretation function to connect the syntactics and semantics. (Halfway done)
+- [x] Define the syntactic category of PTS. Prove that it is contextual.
+- Aim to define an interpretation function to connect the syntactics and semantics.
